x86/AsmFacts.v
@@ -30,8 +30,7 @@ Section WITHMEMORYMODEL.
     match i with
       Pallocframe _ _  
     | Pfreeframe _ _
-    | Pcall_s _ _
-    | Pcall_r _ _ 
+    | Pcall _ _
     | Pret => false
     | _ => true
     end.
@@ -45,39 +44,260 @@ Section WITHMEMORYMODEL.
     forall (ge: Genv.t Asm.fundef unit) rs1 m1 rs2 m2 f init_stk,
       Asm.exec_instr init_stk ge f i rs1 m1 = Next rs2 m2 ->
       rs2 # RSP = rs1 # RSP.
+  
+  Definition written_regs i : list preg :=
+    match i with 
+    (** Moves *)
+    | Pmov_rr rd _
+    | Pmovl_ri rd _ 
+    | Pmovq_ri rd _ 
+    | Pmov_rs rd _
+    | Pmovl_rm rd _ 
+    | Pmovq_rm rd _ => IR rd :: nil
+    | Pmovl_mr a rs 
+    | Pmovq_mr a rs => nil
+    | Pmovsd_ff rd _ 
+    | Pmovsd_fi rd _ 
+    | Pmovsd_fm rd _ => FR rd :: nil
+    | Pmovsd_mf a r1 => nil
+    | Pmovss_fi rd _ 
+    | Pmovss_fm rd _ => FR rd :: nil
+    | Pmovss_mf a r1 => nil
+    | Pfldl_m a  => ST0 :: nil
+    | Pfstpl_m a => ST0 :: nil
+    | Pflds_m a => ST0 :: nil
+    | Pfstps_m a => ST0 :: nil
+    | Pxchg_rr r1 r2 => IR r1 :: IR r2 :: nil
+    (** Moves with conversion *)
+    | Pmovb_mr a rs 
+    | Pmovw_mr a rs => nil
+    | Pmovzb_rr rd _ 
+    | Pmovzb_rm rd _  
+    | Pmovsb_rr rd _ 
+    | Pmovsb_rm rd _  
+    | Pmovzw_rr rd _ 
+    | Pmovzw_rm rd _  
+    | Pmovsw_rr rd _ 
+    | Pmovsw_rm rd _  
+    | Pmovzl_rr rd _ 
+    | Pmovsl_rr rd _ 
+    | Pmovls_rr rd => IR rd :: nil
+    | Pcvtsd2ss_ff rd _ => FR rd :: nil
+    | Pcvtss2sd_ff rd _ => FR rd :: nil
+    | Pcvttsd2si_rf rd _=> IR rd :: nil
+    | Pcvtsi2sd_fr rd _ => FR rd :: nil
+    | Pcvttss2si_rf rd _=> IR rd :: nil
+    | Pcvtsi2ss_fr rd _ => FR rd :: nil
+    | Pcvttsd2sl_rf rd _=> IR rd :: nil
+    | Pcvtsl2sd_fr rd _ => FR rd :: nil
+    | Pcvttss2sl_rf rd _ => IR rd :: nil
+    | Pcvtsl2ss_fr rd _  => FR rd :: nil
+    (* (** Integer arithmetic *) *)
+    | Pleal rd _ 
+    | Pleaq rd _
+    | Pnegl rd
+    | Pnegq rd
+    | Paddl_ri rd _ 
+    | Paddq_ri rd _
+    | Psubl_ri rd _ 
+    | Psubq_ri rd _ 
+    | Psubl_rr rd _
+    | Psubq_rr rd _
+    | Pimull_rr rd _
+    | Pimulq_rr rd _
+    | Pimull_ri rd _ 
+    | Pimulq_ri rd _ => IR rd :: nil
+    | Pimull_r r1 
+    | Pimulq_r r1 
+    | Pmull_r r1  
+    | Pmulq_r r1  => IR RAX :: IR RDX :: nil
+    | Pcltd 
+    | Pcqto => IR RDX :: nil
+    | Pdivl r1  
+    | Pdivq r1  
+    | Pidivl r1 
+    | Pidivq r1 => IR RAX :: IR RDX :: nil
+    | Pandl_rr rd _ 
+    | Pandq_rr rd _ 
+    | Pandl_ri rd _ 
+    | Pandq_ri rd _ 
+    | Porl_rr rd _ 
+    | Porq_rr rd _ 
+    | Porl_ri rd _  
+    | Porq_ri rd _  
+    | Pxorl_r rd
+    | Pxorq_r rd
+    | Pxorl_rr rd _ 
+    | Pxorq_rr rd _ 
+    | Pxorl_ri rd _  
+    | Pxorq_ri rd _  
+    | Pnotl rd 
+    | Pnotq rd 
+    | Psall_rcl rd
+    | Psalq_rcl rd
+    | Psall_ri  rd _     
+    | Psalq_ri  rd _     
+    | Pshrl_rcl rd
+    | Pshrq_rcl rd
+    | Pshrl_ri  rd _     
+    | Pshrq_ri  rd _     
+    | Psarl_rcl rd
+    | Psarq_rcl rd
+    | Psarl_ri  rd _     
+    | Psarq_ri  rd _     
+    | Pshld_ri  rd _ _
+    | Prorl_ri  rd _     
+    | Prorq_ri  rd _     => IR rd :: nil
+    | Pcmpl_rr  _ _    
+    | Pcmpq_rr  _ _    
+    | Pcmpl_ri  _ _    
+    | Pcmpq_ri  _ _    
+    | Ptestl_rr _ _    
+    | Ptestq_rr _ _    
+    | Ptestl_ri _ _    
+    | Ptestq_ri _ _    => nil
+    | Pcmov     c rd _  
+    | Psetcc    c rd    => IR rd :: nil
+    (* (** Floating-point arithmetic *) *)
+    | Paddd_ff   rd _  
+    | Psubd_ff   rd _  
+    | Pmuld_ff   rd _  
+    | Pdivd_ff   rd _  
+    | Pnegd rd 
+    | Pabsd rd => FR rd :: nil
+    | Pcomisd_ff r1 r2  => nil
+    | Pxorpd_f   rd           (**r [xor] with self = set to zero *)
+    | Padds_ff   rd _  
+    | Psubs_ff   rd _  
+    | Pmuls_ff   rd _  
+    | Pdivs_ff   rd _  
+    | Pnegs rd          
+    | Pabss rd          => FR rd :: nil
+    | Pcomiss_ff r1 r2  => nil
+    | Pxorps_f   rd     => FR rd :: nil
+    (* (** Branches and calls *) *)
+    | Pjmp_l _
+    | Pjmp _ _
+    | Pjcc _ _
+    | Pjcc2 _ _ _ => nil
+    | Pjmptbl r tbl => IR RAX :: IR RDX :: nil
+    | Pcall ros sg => nil
+    | Pret => nil
+    (* (** Saving and restoring registers *) *)
+    | Pmov_mr_a _ _   
+    | Pmovsd_mf_a _ _ => nil
+    | Pmov_rm_a rd _   => IR rd :: nil
+    | Pmovsd_fm_a rd _ => FR rd :: nil
 
+    (* (** Pseudo-instructions *) *)
+    | Plabel l => nil
+    | Pallocframe frame ofs_ra (* ofs_link *) => IR RAX :: IR RSP :: nil
+    | Pfreeframe sz ofs_ra (* ofs_link *) => IR RSP :: nil
+    | Pload_parent_pointer rd _ => IR rd :: nil
+    | Pbuiltin ef args res => nil
+    | _ => nil
+    end.
+
+  Require Import AsmRegs.
+
+  Ltac simpl_not_in NIN :=
+    let H1 := fresh in
+    let H2 := fresh in
+    first [ apply Decidable.not_or in NIN; destruct NIN as [H1 H2]; simpl_not_in H2
+          | idtac ].
+
+  Lemma exec_load_rsp:
+    forall F V (ge: _ F V) K m1 am rs1 f0 rs2 m2 sz,
+      exec_load ge K m1 am rs1 f0 sz = Next rs2 m2 ->
+      forall r,
+        ~ In  r (PC :: RA :: CR ZF :: CR CF :: CR PF :: CR SF :: CR OF :: f0 :: nil) ->
+      rs2 r = rs1 r.
+  Proof.
+    intros F V ge' K m1 am rs1 f0 rs2 m2 sz LOAD.
+    unfold exec_load in LOAD. destr_in LOAD. inv LOAD.
+    simpl.
+    unfold nextinstr_nf.
+    intros.
+    simpl_not_in H.
+    simpl. simpl_regs. auto.
+  Qed.
+
+  Lemma exec_store_rsp:
+    forall F V (ge: _ F V)  K m1 am rs1 f0 rs2 m2 (l: list preg) sz,
+      exec_store ge K m1 am rs1 f0 l sz = Next rs2 m2 ->
+      forall r,
+        ~ In  r (PC :: RA :: CR ZF :: CR CF :: CR PF :: CR SF :: CR OF :: l) ->
+      rs2 r = rs1 r.
+  Proof.
+    intros F V ge' K m1 am rs1 f0 rs2 m2 l sz STORE.
+    unfold exec_store in STORE. repeat destr_in STORE.
+    simpl.
+    unfold nextinstr_nf.
+    intros.
+    simpl_not_in H.
+    simpl. simpl_regs. 
+    rewrite Asmgenproof0.undef_regs_other. auto. intros; intro; subst. congruence.
+  Qed.
+  
+  Lemma exec_instr_only_written_regs:
+    forall (ge: Genv.t Asm.fundef unit) rs1 m1 rs2 m2 f i init_stk r,
+      Asm.exec_instr init_stk ge f i rs1 m1 = Next rs2 m2 ->
+      ~ In  r (PC :: RA :: CR ZF :: CR CF :: CR PF :: CR SF :: CR OF :: written_regs i) ->
+      rs2 # r = rs1 # r.
+  Proof.
+    intros ge rs1 m1 rs2 m2 f i init_stk r EI NIN.
+    simpl in NIN.
+    simpl_not_in NIN. rename H7 into NIN.
+    destruct i; simpl in *; repeat destr_in EI;
+      unfold nextinstr_nf, compare_ints, compare_longs, compare_floats, compare_floats32; simpl; simpl_not_in NIN;
+        simpl_regs; eauto;
+          match goal with
+            H: exec_load _ _ _ _ _ _ _ = _ |- _ =>
+            eapply exec_load_rsp; simpl; eauto; intuition
+          | H: exec_store _ _ _ _ _ _ _ _ = _ |- _ =>
+            try now (eapply exec_store_rsp; simpl; eauto; simpl; intuition)
+          | _ => idtac
+          end.
+    repeat destr; simpl_regs; auto.
+    repeat destr; simpl_regs; auto.
+    Ltac solvegl H := unfold goto_label in H; repeat destr_in H; simpl_regs; auto.
+    solvegl H7.
+    solvegl H7.
+    solvegl H7.
+    solvegl H7.
+  Qed.
+
+  Definition check_asm_instr_no_rsp i :=
+    negb (in_dec preg_eq RSP (written_regs i)).
+
+  Definition check_asm_code_no_rsp c : bool :=
+    forallb (fun i => negb (stack_invar i) || check_asm_instr_no_rsp i) c.
+
+  Lemma check_asm_instr_no_rsp_correct i:
+    check_asm_instr_no_rsp i = true ->
+    asm_instr_no_rsp i.
+  Proof.
+    red; intros.
+    eapply exec_instr_only_written_regs. eauto.
+    simpl. intro A. decompose [or] A; try congruence.
+    unfold check_asm_instr_no_rsp in H. unfold proj_sumbool in H. destr_in H. simpl in H. congruence.
+  Qed.
+  
   Definition asm_code_no_rsp (c : Asm.code) : Prop :=
     forall i,
       In i c ->
       asm_instr_no_rsp i.
 
-  Lemma asm_code_no_rsp_cons:
-    forall a l,
-      asm_instr_no_rsp a ->
-      asm_code_no_rsp l ->
-      asm_code_no_rsp (a::l).
+  Lemma check_asm_code_no_rsp_correct c:
+    check_asm_code_no_rsp c = true ->
+    asm_code_no_rsp c.
   Proof.
-    unfold asm_code_no_rsp.
-    intros. simpl in H1. destruct H1; subst; auto.
+    red; intros.
+    unfold check_asm_code_no_rsp in H. rewrite forallb_forall in H.
+    eapply H in H0. destruct (stack_invar i) eqn:STK. simpl in H0. eapply check_asm_instr_no_rsp_correct; eauto.
+    red; congruence.
   Qed.
 
-  Lemma nextinstr_rsp:
-    forall rs sz,
-      nextinstr rs sz RSP = rs RSP.
-  Proof.
-    unfold nextinstr.
-    intros; rewrite Pregmap.gso; congruence.
-  Qed.
-
-  Lemma nextinstr_nf_rsp:
-    forall rs sz,
-      nextinstr_nf rs sz RSP = rs RSP.
-  Proof.
-    unfold nextinstr_nf.
-    intros. rewrite nextinstr_rsp.
-    rewrite Asmgenproof0.undef_regs_other; auto.
-    simpl; intuition subst; congruence. 
-  Qed.
 
   Lemma preg_of_not_rsp:
     forall m x,
@@ -110,273 +330,423 @@ Section WITHMEMORYMODEL.
   Qed.
 
 
-  Lemma compare_floats_rsp:
-    forall a b rs1,
-      compare_floats a b rs1 RSP = rs1 RSP.
-  Proof.
-    unfold compare_floats.
-    intros.
-    destruct a, b; rewrite ?Asmgenproof0.undef_regs_other by simpl; intuition congruence.
-  Qed.
-
-
-  Lemma compare_floats32_rsp:
-    forall a b rs1,
-      compare_floats32 a b rs1 RSP = rs1 RSP.
-  Proof.
-    unfold compare_floats32.
-    intros.
-    destruct a, b; rewrite ?Asmgenproof0.undef_regs_other by simpl; intuition congruence.
-  Qed.
-
-
-  Lemma exec_load_rsp:
-    forall F V (ge: _ F V) K m1 am rs1 f0 rs2 m2 sz,
-      IR RSP <> f0->
-      exec_load ge K m1 am rs1 f0 sz = Next rs2 m2 ->
-      rs2 RSP = rs1 RSP.
-  Proof.
-    intros F V ge' K m1 am rs1 f0 rs2 m2 sz DIFF LOAD.
-    unfold exec_load in LOAD. destr_in LOAD. inv LOAD.
-    rewrite nextinstr_nf_rsp. 
-    rewrite Pregmap.gso. auto. auto. 
-  Qed.
-
-  Lemma exec_store_rsp:
-    forall F V (ge: _ F V)  K m1 am rs1 f0 rs2 m2 (l: list preg) sz, (* preg_of m = f0 -> *)
-      (forall r' : PregEq.t, In r' l -> r' <> RSP) ->
-      exec_store ge K m1 am rs1 f0 l sz = Next rs2 m2 ->
-      rs2 RSP = rs1 RSP.
-  Proof.
-    intros F V ge' K m1 am rs1 f0 rs2 m2 l sz INL STORE.
-    unfold exec_store in STORE. repeat destr_in STORE.
-    rewrite nextinstr_nf_rsp. 
-    rewrite Asmgenproof0.undef_regs_other.
-    auto. intros; apply not_eq_sym. auto.
-  Qed.
-
+  
   Ltac solve_rs:=
-    repeat match goal with
-             H2 : Next _ _ = Next _ _ |- _ =>
-             inv H2
-           | |- _ :preg <> RSP => eapply preg_of_not_rsp; eauto
-           | |- _ :preg<> RSP => eapply ireg_of_not_rsp; eauto
-           | |- _ :preg <> RSP => eapply freg_of_not_rsp; eauto
-           | |- RSP <> _  => apply not_eq_sym
-           | |- _ => rewrite ?nextinstr_nf_rsp, ?nextinstr_rsp, ?compare_floats_rsp, ?compare_floats32_rsp;
-                   try rewrite Pregmap.gso by (apply not_eq_sym; eapply ireg_of_not_rsp; eauto);
-                   try rewrite Pregmap.gso by (apply not_eq_sym; eapply freg_of_not_rsp; eauto);
-                   try reflexivity
+    match goal with
+    | |- not (@eq preg _ (IR RSP)) => solve [ eapply preg_of_not_rsp; eauto
+                                     | eapply ireg_of_not_rsp; eauto
+                                     | eapply freg_of_not_rsp; eauto
+                                     | congruence ]
+    | |- _ => idtac
+    end.
 
+  
+  Lemma loadind_no_rsp:
+    forall ir o t m ti i
+      (IN : In i ti)
+      (TI : loadind ir o t m nil = OK ti),
+      ~ In (IR RSP) (written_regs i).
+  Proof.
+    unfold loadind. intros. monadInv TI. destruct IN. 2: easy. subst.
+    repeat destr_in EQ; simpl; apply Classical_Prop.and_not_or; split; solve_rs; auto.
+  Qed.
+
+  Lemma storeind_no_rsp:
+    forall ir o t m ti i
+      (IN : In i ti)
+      (TI : storeind ir o t m nil = OK ti),
+      ~ In (IR RSP) (written_regs i).
+  Proof.
+    unfold storeind. intros. monadInv TI. destruct IN. 2: easy. subst.
+    repeat destr_in EQ; simpl; try apply Classical_Prop.and_not_or; try split; solve_rs; auto.
+  Qed.
+
+  Ltac solve_in_regs :=
+    repeat match goal with
+           | H: mk_mov _ _ _ = _ |- _ => unfold mk_mov in H; repeat destr_in H
+           | H: OK _ = OK _ |- _ => inv H
+           | H: mk_intconv _ _ _ _ = _ |- _ => unfold mk_intconv in H
+           | H: bind _ _ = _ |- _ => monadInv H
+           | IN: In _ (_ :: _) |- _ => destruct IN as [IN | IN]; inv IN; simpl in *
+           | IN: In _ (_ ++ _) |- _ => rewrite in_app in IN; destruct IN as [IN|IN]
+           | OR: _ \/ _ |- _ => destruct OR as [OR|OR]; inv OR; simpl
+           | |- ~ (_ \/ _) => apply Classical_Prop.and_not_or
+           | |- ~ _ /\ ~ _ => split; auto
+           | H: False |- _ => destruct H
+           | H: In _ nil |- _ => destruct H
+           | IN: In _ _ |- _ => repeat destr_in IN; simpl in *
+           | _ => simpl in *; solve_rs; auto
            end.
 
-
-  Lemma loadind_no_change_rsp:
-    forall i t m x0 x1 r,
-      asm_code_no_rsp x0 ->
-      loadind r i t m x0 = OK x1 ->
-      asm_code_no_rsp x1.
-  Proof.
-    intros i t m x0 x1 r IH EQ.
-    unfold loadind in EQ. unfold Asmgen.loadind in EQ.
-    simpl in EQ.
-    repeat destr_in EQ; apply asm_code_no_rsp_cons; auto; red; simpl;
-    intros ge rs1 m1 rs2 m2 ff init_stk EI; unfold exec_instr in EI; simpl in EI;
-      eapply exec_load_rsp; eauto; apply not_eq_sym; solve_rs.
-  Qed.
-
-  Lemma storeind_no_change_rsp:
-    forall i t m x0 x1 r,
-      asm_code_no_rsp x0 ->
-      storeind m r i t x0 = OK x1 ->
-      asm_code_no_rsp x1.
-  Proof.
-    intros i t m x0 x1 r IH EQ.
-    unfold storeind in EQ. unfold Asmgen.storeind in EQ.
-    repeat destr_in EQ; apply asm_code_no_rsp_cons; auto; red; simpl;
-      intros ge rs1 m1 rs2 m2 ff init_stk EI; unfold exec_instr in EI; simpl in EI;
-      eapply exec_store_rsp; eauto; simpl; intuition subst; congruence.
-  Qed.
-
-  Lemma mk_move_nochange_rsp:
-    forall x0 x1 m m0,
-      asm_code_no_rsp x0 ->
-      mk_mov (preg_of m) (preg_of m0) x0 = OK x1 ->
-      asm_code_no_rsp x1.
-  Proof.
-    intros x0 x1 m m0 A B.
-    unfold mk_mov in B. unfold Asmgen.mk_mov in B.
-    repeat destr_in B; apply asm_code_no_rsp_cons; auto; red; simpl; intros;
-      inv H0; rewrite nextinstr_rsp;
-        rewrite Pregmap.gso; auto;
-          apply not_eq_sym; eapply preg_of_not_rsp; eauto.
-  Qed.  
-  
-  Ltac invasm :=
-    repeat match goal with
-             H: bind _ ?x = OK ?x1 |- _ =>
-             monadInv H
-           | H: exec_instr ?init_stk _ _ _ _ _ = _ |- _ =>
-             unfold exec_instr in H; simpl in H; inv H
-           | |- _ => apply asm_code_no_rsp_cons; auto; red; simpl; intros; solve_rs
-           end.
-
-  Lemma mkset_cc_no_rsp:
-    forall x0 m x2 i c,
-      asm_code_no_rsp x0 ->
-      In i (mk_setcc c x2 x0) ->
-      Asmgen.ireg_of m = OK x2 ->
-      asm_instr_no_rsp i.
-  Proof.
-    intros x0 m x2 i c A B C.
-    Ltac ainr :=
-      match goal with
-        |- asm_instr_no_rsp ?i =>
-        let invar := fresh "invar" in
-        (* let F := fresh "F" in *)
-        (* let V := fresh "V" in *)
-        let ge := fresh "ge" in
-        let rs1 := fresh "rs1" in
-        let m1 := fresh "m1" in
-        let rs2 := fresh "rs2" in
-        let m2 := fresh "m2" in
-        let init_stk := fresh "init_stk" in
-        let EI := fresh "EI" in
-        intros invar ge rs1 m1 rs2 m2 f init_stk EI;
-        unfold Asm.exec_instr in EI; simpl in EI; solve_rs
-      end.
-    unfold mk_setcc in B. unfold Asmgen.mk_setcc in B.
-    destr_in B; destruct c; simpl in *;
-      unfold Asmgen.mk_setcc_base in *; simpl in *;
-        (intuition subst; simpl in *; eauto; try now ainr).
-    - destr_in B; simpl in *; intuition subst; simpl in *; auto; try ainr.
-    - destr_in B; simpl in *; intuition subst; simpl in *; auto; try ainr.
-  Qed.
-
-  Lemma asmgen_transl_cond_rsp:
-    forall x0 m x2 x1 cond l,
-      asm_code_no_rsp x0 ->
-      Asmgen.ireg_of m = OK x2 ->
-      transl_cond cond l (mk_setcc (Asmgen.testcond_for_condition cond) x2 x0) = OK x1 ->
-      asm_code_no_rsp x1.
-  Proof.
-    unfold transl_cond, Asmgen.transl_cond; simpl.
-    intros x0 m x2 x1 cond l ACNR IREG TRANSL.
-    repeat destr_in TRANSL; try destruct (c:comparison);
-      invasm; eauto;
-        simpl in *; solve_rs; eauto using mkset_cc_no_rsp.
-  Qed.
-
-  Lemma goto_label_rsp:
-    forall (ge: Genv.t Asm.fundef unit) rs1 rs2 f l m1 m2,
-      goto_label ge f l rs1 m1 = Next rs2 m2 ->
-      rs2 RSP = rs1 RSP.
-  Proof.
-    unfold goto_label.
-    intros ge rs1 rs2 f l m1 m2 A.
-    repeat destr_in A. solve_rs.
-  Qed.
-
-  Lemma mkjcc_no_rsp:
-    forall x0 x2 i c,
-      asm_code_no_rsp x0 ->
-      In i (mk_jcc c x2 x0) ->
-      asm_instr_no_rsp i.
-  Proof.
-    intros x0 x2 i c A H1.
-    unfold mk_jcc in H1.
-    destr_in H1; simpl in *; intuition subst; simpl in *; eauto; ainr;
-      repeat destr_in EI; eauto using goto_label_rsp.
-  Qed.
-  
-  Lemma asmgen_transl_cond_rsp':
-    forall x0 x2 x1 cond l,
-      asm_code_no_rsp x0 ->
-      transl_cond cond l (mk_jcc (Asmgen.testcond_for_condition cond) x2 x0) = OK x1 ->
-      asm_code_no_rsp x1.
-  Proof.
-    unfold transl_cond; simpl.
-    intros x0 x2 x1 cond l ACNR TRANSL.
-    repeat destr_in TRANSL;
-      try destruct (c: comparison);
-      invasm; eauto; intuition subst; eauto; try solve_rs;
-        ainr; repeat destr_in EI; eauto using goto_label_rsp.
-  Qed.
-
-  Lemma intconv_no_change_rsp:
-    forall x0
-      (ACNR : asm_code_no_rsp x0)
-      m x3
-      (IREG: Asmgen.ireg_of m = OK x3)
-      x2 x1 i
-      (REC: forall x2,  asm_instr_no_rsp ((i x3 x2)))
-      (CONV: Asmgen.mk_intconv i x3 x2 x0 = OK x1),
-      asm_code_no_rsp x1.
+  Lemma transl_cond_no_rsp:
+    forall cond l c c' i
+      (INV: stack_invar i = true)
+      (TC : transl_cond cond l c = OK c')
+      (IN: In i c'),
+      ~ In (IR RSP) (written_regs i) \/ In i c.
   Proof.
     intros.
-    unfold Asmgen.mk_intconv in CONV. inv CONV.
-    destr; repeat apply asm_code_no_rsp_cons; auto.
-    red; simpl; intros; invasm; solve_rs.
+    destruct cond; simpl in TC; repeat destr_in TC; simpl;
+      unfold mk_setcc, mk_setcc_base in *; simpl in *;
+        solve_in_regs; simpl; auto.
+    unfold floatcomp; destr; solve_in_regs.
+    unfold floatcomp; destr; solve_in_regs.
+    unfold floatcomp32; destr; solve_in_regs.
+    unfold floatcomp32; destr; solve_in_regs.
   Qed.
 
+  Lemma transl_op_no_rsp:
+    forall op l r c' i
+      (INV: stack_invar i = true)
+      (TC : transl_op op l r nil = OK c')
+      (IN: In i c'),
+      ~ In (IR RSP) (written_regs i).
+  Proof.
+    intros.
+    destruct op; simpl in TC; repeat destr_in TC; simpl; solve_in_regs.
+    eapply transl_cond_no_rsp in EQ0; eauto.
+    destruct EQ0; auto. 
+    unfold mk_setcc, mk_setcc_base in *; simpl in *.
+    solve_in_regs; solve_rs.
+  Qed.
+
+  Lemma transl_code_no_rsp:
+    forall f c b c' i
+      (INV: stack_invar i = true)
+      (TC : transl_code f c b = OK c')
+      (IN: In i c'),
+      ~ In (IR RSP) (written_regs i).
+  Proof.
+    induction c; simpl; intros; eauto. inv TC. easy.
+    monadInv TC.
+    edestruct transl_instr_eq as (ti & TI & EQti). eauto. subst.
+    rewrite in_app in IN.
+    destruct IN as [IN|IN]; eauto.
+    clear EQ EQ0.
+    destruct a; simpl in TI; repeat destr_in TI; eauto using loadind_no_rsp, storeind_no_rsp.
+    - monadInv H0. simpl in IN. destruct IN as [IN|IN]. inv IN. simpl. intuition congruence.
+      eapply loadind_no_rsp; eauto.
+    - eapply transl_op_no_rsp; eauto.
+    - unfold transl_load in H0. solve_in_regs.
+      repeat destr_in EQ1; solve_in_regs.
+    - unfold transl_store in H0. solve_in_regs.
+      repeat destr_in EQ0; solve_in_regs; auto.
+      inv EQ1; solve_in_regs; auto.
+      inv EQ1; solve_in_regs; auto.
+    - solve_in_regs.
+    - solve_in_regs.
+    - solve_in_regs.
+    - solve_in_regs.
+    - solve_in_regs.
+    - solve_in_regs.
+    - solve_in_regs.
+    - eapply transl_cond_no_rsp in H0 ; eauto. destruct H0; auto.
+      unfold mk_jcc in *; simpl in *.
+      solve_in_regs; solve_rs; auto.
+    - solve_in_regs.
+    - solve_in_regs.
+  Qed.
+  
   Lemma asmgen_no_change_rsp:
     forall f tf,
       transf_function f = OK tf ->
-      asm_code_no_rsp (Asm.fn_code tf).
+      check_asm_code_no_rsp (fn_code tf) = true.
   Proof.
-    intros f tf TR.
-    unfold transf_function, Asmgen.transf_function in TR.
-    monadInv TR.
-    destr_in EQ0. inv EQ0.
-    unfold transl_function in EQ.
-    monadInv EQ. simpl.
-    apply asm_code_no_rsp_cons. red; simpl. congruence.
-    unfold transl_code' in EQ0.
-    revert EQ0.
-    set (P := fun f => forall x y, f x = OK y -> asm_code_no_rsp x -> asm_code_no_rsp y).
-    assert (POK: P (fun c => OK c)).
-    { unfold P; simpl. inversion 1; tauto. }
-    revert POK.
-    generalize (Mach.fn_code f) true (fun c : code => OK c).
-    clear g.
-    induction c; simpl; intros; eauto.
-    eapply POK; eauto. red; easy.
-    eapply IHc. 2: apply EQ0.
-    unfold P. intros x0 y BIND ACNR. monadInv BIND.
-    eapply POK; eauto.
-
-    Ltac t :=
-      match goal with
-      | EQ: context [match ?a with _ => _ end] |- _ => destr_in EQ
-      | EQ: loadind _ _ _ _ _ = OK ?x |- asm_code_no_rsp ?x => eapply loadind_no_change_rsp in EQ; eauto
-      | EQ: Asmgen.storeind _ _ _ _ _ = OK ?x |- asm_code_no_rsp ?x => eapply storeind_no_change_rsp in EQ; eauto
-      | EQ: Asmgen.mk_intconv _ _ _ _ = OK ?x |- asm_code_no_rsp ?x => eapply intconv_no_change_rsp in EQ; eauto
-      | EQ: bind _ _ = OK _ |- _ => monadInv EQ
-      | EQ: OK _ = OK _ |- _ => inv EQ
-      | |- asm_instr_no_rsp _ => now (red; simpl; intros; invasm; solve_rs)
-      | |- asm_code_no_rsp (_ :: _) => eapply asm_code_no_rsp_cons;[red; simpl; intros; invasm; repeat t; solve_rs|eauto]
-      | |- _ => intros
-      end.
-    Hint Resolve not_eq_sym ireg_of_not_rsp freg_of_not_rsp.
-    destruct a; simpl in EQ; repeat (t; simpl).
-    - unfold Asmgen.transl_op in EQ.
-      repeat destr_in EQ; repeat t; try now (invasm; solve_rs).
-      + eapply mk_move_nochange_rsp; eauto.
-      + repeat (t; simpl).
-      + eapply asmgen_transl_cond_rsp; eauto.
-    - unfold Asmgen.transl_load in EQ.
-      repeat t; eapply exec_load_rsp; eauto.
-    - unfold Asmgen.transl_store in EQ.
-      repeat t; try eapply exec_store_rsp; eauto; try easy.
-      unfold Asmgen.mk_storebyte in EQ4. inv EQ4.
-      repeat (t; simpl); eapply exec_store_rsp; eauto; easy.
-      unfold Asmgen.mk_storebyte in EQ4. inv EQ4.
-      repeat (t; simpl); eapply exec_store_rsp; eauto; easy.
-    - inv H0.
-    - repeat t. eapply goto_label_rsp; eauto.
-    - eapply asmgen_transl_cond_rsp'; eauto.
-    - erewrite goto_label_rsp. 2: eauto. solve_rs.
+    unfold check_asm_code_no_rsp.
+    intros. rewrite forallb_forall.
+    unfold check_asm_instr_no_rsp.
+    unfold proj_sumbool.
+    intros. destruct (stack_invar x) eqn:INV. simpl.
+    destr. exfalso.
+    monadInv H. repeat destr_in EQ0.
+    monadInv EQ. simpl in *.
+    destruct H0. subst. simpl in *. congruence.
+    rewrite Asmgenproof0.transl_code'_transl_code in EQ0.
+    eapply transl_code_no_rsp in EQ0; eauto. simpl. auto.
   Qed.
+
+      
+  (* Lemma asm_code_no_rsp_cons: *)
+  (*   forall a l, *)
+  (*     asm_instr_no_rsp a -> *)
+  (*     asm_code_no_rsp l -> *)
+  (*     asm_code_no_rsp (a::l). *)
+  (* Proof. *)
+  (*   unfold asm_code_no_rsp. *)
+  (*   intros. simpl in H1. destruct H1; subst; auto. *)
+  (* Qed. *)
+
+  (* Lemma nextinstr_rsp: *)
+  (*   forall rs sz, *)
+  (*     nextinstr rs sz RSP = rs RSP. *)
+  (* Proof. *)
+  (*   unfold nextinstr. *)
+  (*   intros; rewrite Pregmap.gso; congruence. *)
+  (* Qed. *)
+
+  (* Lemma nextinstr_nf_rsp: *)
+  (*   forall rs sz, *)
+  (*     nextinstr_nf rs sz RSP = rs RSP. *)
+  (* Proof. *)
+  (*   unfold nextinstr_nf. *)
+  (*   intros. rewrite nextinstr_rsp. *)
+  (*   rewrite Asmgenproof0.undef_regs_other; auto. *)
+  (*   simpl; intuition subst; congruence.  *)
+  (* Qed. *)
+
+  (* Lemma compare_floats_rsp: *)
+  (*   forall a b rs1, *)
+  (*     compare_floats a b rs1 RSP = rs1 RSP. *)
+  (* Proof. *)
+  (*   unfold compare_floats. *)
+  (*   intros. *)
+  (*   destruct a, b; rewrite ?Asmgenproof0.undef_regs_other by simpl; intuition congruence. *)
+  (* Qed. *)
+
+
+  (* Lemma compare_floats32_rsp: *)
+  (*   forall a b rs1, *)
+  (*     compare_floats32 a b rs1 RSP = rs1 RSP. *)
+  (* Proof. *)
+  (*   unfold compare_floats32. *)
+  (*   intros. *)
+  (*   destruct a, b; rewrite ?Asmgenproof0.undef_regs_other by simpl; intuition congruence. *)
+  (* Qed. *)
+
+
+  (* Lemma exec_load_rsp: *)
+  (*   forall F V (ge: _ F V) K m1 am rs1 f0 rs2 m2 sz, *)
+  (*     IR RSP <> f0-> *)
+  (*     exec_load ge K m1 am rs1 f0 sz = Next rs2 m2 -> *)
+  (*     rs2 RSP = rs1 RSP. *)
+  (* Proof. *)
+  (*   intros F V ge' K m1 am rs1 f0 rs2 m2 sz DIFF LOAD. *)
+  (*   unfold exec_load in LOAD. destr_in LOAD. inv LOAD. *)
+  (*   rewrite nextinstr_nf_rsp.  *)
+  (*   rewrite Pregmap.gso. auto. auto.  *)
+  (* Qed. *)
+
+  (* Lemma exec_store_rsp: *)
+  (*   forall F V (ge: _ F V)  K m1 am rs1 f0 rs2 m2 (l: list preg) sz, (* preg_of m = f0 -> *) *)
+  (*     (forall r' : PregEq.t, In r' l -> r' <> RSP) -> *)
+  (*     exec_store ge K m1 am rs1 f0 l sz = Next rs2 m2 -> *)
+  (*     rs2 RSP = rs1 RSP. *)
+  (* Proof. *)
+  (*   intros F V ge' K m1 am rs1 f0 rs2 m2 l sz INL STORE. *)
+  (*   unfold exec_store in STORE. repeat destr_in STORE. *)
+  (*   rewrite nextinstr_nf_rsp.  *)
+  (*   rewrite Asmgenproof0.undef_regs_other. *)
+  (*   auto. intros; apply not_eq_sym. auto. *)
+  (* Qed. *)
+
+
+
+  (* Lemma loadind_no_change_rsp: *)
+  (*   forall i t m x0 x1 r, *)
+  (*     asm_code_no_rsp x0 -> *)
+  (*     loadind r i t m x0 = OK x1 -> *)
+  (*     asm_code_no_rsp x1. *)
+  (* Proof. *)
+  (*   intros i t m x0 x1 r IH EQ. *)
+  (*   unfold loadind in EQ. unfold Asmgen.loadind in EQ. *)
+  (*   simpl in EQ. *)
+  (*   repeat destr_in EQ; apply asm_code_no_rsp_cons; auto; red; simpl; *)
+  (*   intros ge rs1 m1 rs2 m2 ff init_stk EI; unfold exec_instr in EI; simpl in EI; *)
+  (*     eapply exec_load_rsp; eauto; apply not_eq_sym; solve_rs. *)
+  (* Qed. *)
+
+  (* Lemma storeind_no_change_rsp: *)
+  (*   forall i t m x0 x1 r, *)
+  (*     asm_code_no_rsp x0 -> *)
+  (*     storeind m r i t x0 = OK x1 -> *)
+  (*     asm_code_no_rsp x1. *)
+  (* Proof. *)
+  (*   intros i t m x0 x1 r IH EQ. *)
+  (*   unfold storeind in EQ. unfold Asmgen.storeind in EQ. *)
+  (*   repeat destr_in EQ; apply asm_code_no_rsp_cons; auto; red; simpl; *)
+  (*     intros ge rs1 m1 rs2 m2 ff init_stk EI; unfold exec_instr in EI; simpl in EI; *)
+  (*     eapply exec_store_rsp; eauto; simpl; intuition subst; congruence. *)
+  (* Qed. *)
+
+  (* Lemma mk_move_nochange_rsp: *)
+  (*   forall x0 x1 m m0, *)
+  (*     asm_code_no_rsp x0 -> *)
+  (*     mk_mov (preg_of m) (preg_of m0) x0 = OK x1 -> *)
+  (*     asm_code_no_rsp x1. *)
+  (* Proof. *)
+  (*   intros x0 x1 m m0 A B. *)
+  (*   unfold mk_mov in B. unfold Asmgen.mk_mov in B. *)
+  (*   repeat destr_in B; apply asm_code_no_rsp_cons; auto; red; simpl; intros; *)
+  (*     inv H0; rewrite nextinstr_rsp; *)
+  (*       rewrite Pregmap.gso; auto; *)
+  (*         apply not_eq_sym; eapply preg_of_not_rsp; eauto. *)
+  (* Qed.   *)
+  
+  (* Ltac invasm := *)
+  (*   repeat match goal with *)
+  (*            H: bind _ ?x = OK ?x1 |- _ => *)
+  (*            monadInv H *)
+  (*          | H: exec_instr ?init_stk _ _ _ _ _ = _ |- _ => *)
+  (*            unfold exec_instr in H; simpl in H; inv H *)
+  (*          | |- _ => apply asm_code_no_rsp_cons; auto; red; simpl; intros; solve_rs *)
+  (*          end. *)
+
+  (* Lemma mkset_cc_no_rsp: *)
+  (*   forall x0 m x2 i c, *)
+  (*     asm_code_no_rsp x0 -> *)
+  (*     In i (mk_setcc c x2 x0) -> *)
+  (*     Asmgen.ireg_of m = OK x2 -> *)
+  (*     asm_instr_no_rsp i. *)
+  (* Proof. *)
+  (*   intros x0 m x2 i c A B C. *)
+  (*   Ltac ainr := *)
+  (*     match goal with *)
+  (*       |- asm_instr_no_rsp ?i => *)
+  (*       let invar := fresh "invar" in *)
+  (*       (* let F := fresh "F" in *) *)
+  (*       (* let V := fresh "V" in *) *)
+  (*       let ge := fresh "ge" in *)
+  (*       let rs1 := fresh "rs1" in *)
+  (*       let m1 := fresh "m1" in *)
+  (*       let rs2 := fresh "rs2" in *)
+  (*       let m2 := fresh "m2" in *)
+  (*       let init_stk := fresh "init_stk" in *)
+  (*       let EI := fresh "EI" in *)
+  (*       intros invar ge rs1 m1 rs2 m2 f init_stk EI; *)
+  (*       unfold Asm.exec_instr in EI; simpl in EI; solve_rs *)
+  (*     end. *)
+  (*   unfold mk_setcc in B. unfold Asmgen.mk_setcc in B. *)
+  (*   destr_in B; destruct c; simpl in *; *)
+  (*     unfold Asmgen.mk_setcc_base in *; simpl in *; *)
+  (*       (intuition subst; simpl in *; eauto; try now ainr). *)
+  (*   - destr_in B; simpl in *; intuition subst; simpl in *; auto; try ainr. *)
+  (*   - destr_in B; simpl in *; intuition subst; simpl in *; auto; try ainr. *)
+  (* Qed. *)
+
+  (* Lemma asmgen_transl_cond_rsp: *)
+  (*   forall x0 m x2 x1 cond l, *)
+  (*     asm_code_no_rsp x0 -> *)
+  (*     Asmgen.ireg_of m = OK x2 -> *)
+  (*     transl_cond cond l (mk_setcc (Asmgen.testcond_for_condition cond) x2 x0) = OK x1 -> *)
+  (*     asm_code_no_rsp x1. *)
+  (* Proof. *)
+  (*   unfold transl_cond, Asmgen.transl_cond; simpl. *)
+  (*   intros x0 m x2 x1 cond l ACNR IREG TRANSL. *)
+  (*   repeat destr_in TRANSL; try destruct (c:comparison); *)
+  (*     invasm; eauto; *)
+  (*       simpl in *; solve_rs; eauto using mkset_cc_no_rsp. *)
+  (* Qed. *)
+
+  (* Lemma goto_label_rsp: *)
+  (*   forall (ge: Genv.t Asm.fundef unit) rs1 rs2 f l m1 m2, *)
+  (*     goto_label ge f l rs1 m1 = Next rs2 m2 -> *)
+  (*     rs2 RSP = rs1 RSP. *)
+  (* Proof. *)
+  (*   unfold goto_label. *)
+  (*   intros ge rs1 rs2 f l m1 m2 A. *)
+  (*   repeat destr_in A. solve_rs. *)
+  (* Qed. *)
+
+  (* Lemma mkjcc_no_rsp: *)
+  (*   forall x0 x2 i c, *)
+  (*     asm_code_no_rsp x0 -> *)
+  (*     In i (mk_jcc c x2 x0) -> *)
+  (*     asm_instr_no_rsp i. *)
+  (* Proof. *)
+  (*   intros x0 x2 i c A H1. *)
+  (*   unfold mk_jcc in H1. *)
+  (*   destr_in H1; simpl in *; intuition subst; simpl in *; eauto; ainr; *)
+  (*     repeat destr_in EI; eauto using goto_label_rsp. *)
+  (* Qed. *)
+  
+  (* Lemma asmgen_transl_cond_rsp': *)
+  (*   forall x0 x2 x1 cond l, *)
+  (*     asm_code_no_rsp x0 -> *)
+  (*     transl_cond cond l (mk_jcc (Asmgen.testcond_for_condition cond) x2 x0) = OK x1 -> *)
+  (*     asm_code_no_rsp x1. *)
+  (* Proof. *)
+  (*   unfold transl_cond; simpl. *)
+  (*   intros x0 x2 x1 cond l ACNR TRANSL. *)
+  (*   repeat destr_in TRANSL; *)
+  (*     try destruct (c: comparison); *)
+  (*     invasm; eauto; intuition subst; eauto; try solve_rs; *)
+  (*       ainr; repeat destr_in EI; eauto using goto_label_rsp. *)
+  (* Qed. *)
+
+  (* Lemma intconv_no_change_rsp: *)
+  (*   forall x0 *)
+  (*     (ACNR : asm_code_no_rsp x0) *)
+  (*     m x3 *)
+  (*     (IREG: Asmgen.ireg_of m = OK x3) *)
+  (*     x2 x1 i *)
+  (*     (REC: forall x2,  asm_instr_no_rsp ((i x3 x2))) *)
+  (*     (CONV: Asmgen.mk_intconv i x3 x2 x0 = OK x1), *)
+  (*     asm_code_no_rsp x1. *)
+  (* Proof. *)
+  (*   intros. *)
+  (*   unfold Asmgen.mk_intconv in CONV. inv CONV. *)
+  (*   destr; repeat apply asm_code_no_rsp_cons; auto. *)
+  (*   red; simpl; intros; invasm; solve_rs. *)
+  (* Qed. *)
+
+  (* Lemma asmgen_no_change_rsp: *)
+  (*   forall f tf, *)
+  (*     transf_function f = OK tf -> *)
+  (*     asm_code_no_rsp (Asm.fn_code tf). *)
+  (* Proof. *)
+  (*   intros f tf TR. *)
+  (*   unfold transf_function, Asmgen.transf_function in TR. *)
+  (*   monadInv TR. *)
+  (*   destr_in EQ0. inv EQ0. *)
+  (*   unfold transl_function in EQ. *)
+  (*   monadInv EQ. simpl. *)
+  (*   apply asm_code_no_rsp_cons. red; simpl. congruence. *)
+  (*   unfold transl_code' in EQ0. *)
+  (*   revert EQ0. *)
+  (*   set (P := fun f => forall x y, f x = OK y -> asm_code_no_rsp x -> asm_code_no_rsp y). *)
+  (*   assert (POK: P (fun c => OK c)). *)
+  (*   { unfold P; simpl. inversion 1; tauto. } *)
+  (*   revert POK. *)
+  (*   generalize (Mach.fn_code f) true (fun c : code => OK c). *)
+  (*   clear g. *)
+  (*   induction c; simpl; intros; eauto. *)
+  (*   eapply POK; eauto. red; easy. *)
+  (*   eapply IHc. 2: apply EQ0. *)
+  (*   unfold P. intros x0 y BIND ACNR. monadInv BIND. *)
+  (*   eapply POK; eauto. *)
+
+  (*   Ltac t := *)
+  (*     match goal with *)
+  (*     | EQ: context [match ?a with _ => _ end] |- _ => destr_in EQ *)
+  (*     | EQ: loadind _ _ _ _ _ = OK ?x |- asm_code_no_rsp ?x => eapply loadind_no_change_rsp in EQ; eauto *)
+  (*     | EQ: Asmgen.storeind _ _ _ _ _ = OK ?x |- asm_code_no_rsp ?x => eapply storeind_no_change_rsp in EQ; eauto *)
+  (*     | EQ: Asmgen.mk_intconv _ _ _ _ = OK ?x |- asm_code_no_rsp ?x => eapply intconv_no_change_rsp in EQ; eauto *)
+  (*     | EQ: bind _ _ = OK _ |- _ => monadInv EQ *)
+  (*     | EQ: OK _ = OK _ |- _ => inv EQ *)
+  (*     | |- asm_instr_no_rsp _ => now (red; simpl; intros; invasm; solve_rs) *)
+  (*     | |- asm_code_no_rsp (_ :: _) => eapply asm_code_no_rsp_cons;[red; simpl; intros; invasm; repeat t; solve_rs|eauto] *)
+  (*     | |- _ => intros *)
+  (*     end. *)
+  (*   Hint Resolve not_eq_sym ireg_of_not_rsp freg_of_not_rsp. *)
+  (*   destruct a; simpl in EQ; repeat (t; simpl). *)
+  (*   - unfold Asmgen.transl_op in EQ. *)
+  (*     repeat destr_in EQ; repeat t; try now (invasm; solve_rs). *)
+  (*     + eapply mk_move_nochange_rsp; eauto. *)
+  (*     + repeat (t; simpl). *)
+  (*     + eapply asmgen_transl_cond_rsp; eauto. *)
+  (*   - unfold Asmgen.transl_load in EQ. *)
+  (*     repeat t; eapply exec_load_rsp; eauto. *)
+  (*   - unfold Asmgen.transl_store in EQ. *)
+  (*     repeat t; try eapply exec_store_rsp; eauto; try easy. *)
+  (*     unfold Asmgen.mk_storebyte in EQ4. inv EQ4. *)
+  (*     repeat (t; simpl); eapply exec_store_rsp; eauto; easy. *)
+  (*     unfold Asmgen.mk_storebyte in EQ4. inv EQ4. *)
+  (*     repeat (t; simpl); eapply exec_store_rsp; eauto; easy. *)
+  (*   - inv H0. *)
+  (*   - repeat t. eapply goto_label_rsp; eauto. *)
+  (*   - eapply asmgen_transl_cond_rsp'; eauto. *)
+  (*   - erewrite goto_label_rsp. 2: eauto. solve_rs. *)
+  (* Qed. *)
 
   Definition asm_instr_no_stack (i : Asm.instruction) : Prop :=
     stack_invar i = true ->
@@ -628,7 +998,6 @@ Section WITHMEMORYMODEL.
               | idtac
               ].
       apply Mem.strong_unchanged_on_weak, Mem.push_new_stage_unchanged_on.
-      apply Mem.strong_unchanged_on_weak, Mem.push_new_stage_unchanged_on.
       apply Mem.strong_unchanged_on_weak, Mem.unrecord_stack_block_unchanged_on; auto.
       - eapply Mem.unchanged_on_trans.
         eapply Mem.alloc_unchanged_on; eauto.
@@ -665,7 +1034,6 @@ Section WITHMEMORYMODEL.
       - unfold stack_invar in INVAR. unfold exec_instr in EI.
         set (AA := i).
         destr_in INVAR; simpl in *; repeat destr_in EI; repeat rewrite_stack_blocks; rewrite ? STK; eauto.
-        + exists ((None,nil)::l); auto.
         + exists ((None,nil)::l); auto.
         + inv t. rewrite STK in H.
           destruct l; simpl; eauto. simpl in *.
