x86/RealAsm.v
@@ -13,7 +13,617 @@ Require Import Globalenvs.
 Require Import Events.
 Require Import Values.
 Require Import Conventions1.
-Require Import RawAsm.
+Require Import RawAsm AsmFacts AsmRegs.
+
+Section WFASM.
+
+
+  Fixpoint in_builtin_arg (b: builtin_arg preg) (r: preg) :=
+    match b with
+    | BA x => if preg_eq r x then True else False
+    | BA_splitlong ba1 ba2 => in_builtin_arg ba1 r \/ in_builtin_arg ba2 r
+    | _ => False
+    end.
+
+  Inductive is_alloc : instruction -> Prop :=
+    is_alloc_intro f sz:
+      is_alloc (Pallocframe f sz).
+
+  Definition make_palloc f : instruction :=
+    let sz := frame_size f in 
+    (Pallocframe f (Ptrofs.sub (Ptrofs.repr (align sz 8)) (Ptrofs.repr (size_chunk Mptr)))).
+
+  Lemma make_palloc_is_alloc:
+    forall f,
+      is_alloc (make_palloc f).
+  Proof. constructor. Qed.
+  
+  Inductive is_free : instruction -> Prop :=
+    is_free_intro sz ora:
+      is_free (Pfreeframe sz ora).
+
+  Lemma is_free_dec:
+    forall i,
+      {is_free i} + {~ is_free i}.
+  Proof.
+    destruct i; try now (right; intro A; inv A).
+    left. econstructor; eauto.
+  Defined.
+  
+  Inductive is_jmp: instruction -> Prop :=
+  | is_jmp_intro:
+      forall ros sg,
+        is_jmp (Pjmp ros sg).
+
+  Inductive intermediate_instruction : instruction -> Prop :=
+  | ii_alloc i: is_alloc i -> intermediate_instruction i
+  | ii_jmp i: i = Pret \/ is_jmp i -> intermediate_instruction i.
+
+  Record wf_asm_function (f: function): Prop :=
+    {
+
+      wf_asm_alloc_only_at_beginning:
+        forall o fi ora,
+          find_instr o (fn_code f) = Some (Pallocframe fi ora) ->
+          o = 0;
+
+      wf_asm_alloc_at_beginning:
+        find_instr 0 (fn_code f) = Some (make_palloc (fn_frame f));
+
+      wf_asm_after_freeframe:
+        forall i o,
+          find_instr (Ptrofs.unsigned o) (fn_code f) = Some i ->
+          is_free i ->
+          exists i' ,
+            find_instr (Ptrofs.unsigned (Ptrofs.add o (Ptrofs.repr (instr_size i)))) (fn_code f) = Some i' /\
+            (i' = Pret \/ is_jmp i' );
+
+      wf_asm_ret_jmp_comes_after_freeframe:
+        forall i o,
+          find_instr (Ptrofs.unsigned o) (fn_code f) = Some i ->
+          i = Pret \/ is_jmp i ->
+          exists o' ifree,
+            find_instr (Ptrofs.unsigned o') (fn_code f) = Some ifree /\
+            is_free ifree /\
+            Ptrofs.unsigned o' + instr_size ifree = Ptrofs.unsigned o;
+
+      wf_asm_code_bounded:
+        0 <= code_size (fn_code f) <= Ptrofs.max_unsigned;
+
+      wf_asm_builtin_not_PC:
+        forall o ef args res,
+          find_instr o (fn_code f) = Some (Pbuiltin ef args res) ->
+          ~ in_builtin_res res PC /\
+          ~ in_builtin_res res RSP
+          /\ Forall (fun arg : builtin_arg preg => ~ in_builtin_arg arg RA) args;
+
+      wf_asm_jmp_no_rsp:
+        forall o (r: ireg) sg,
+          find_instr o (fn_code f) = Some (Pjmp (inl r) sg) ->
+          r <> RSP;
+
+      wf_asm_call_no_rsp:
+        forall o (r: ireg) sg,
+          find_instr o (fn_code f) = Some (Pcall (inl r) sg) ->
+          r <> RSP;
+      
+      wf_asm_free_spec:
+        forall o sz ora,
+          find_instr o (fn_code f) = Some (Pfreeframe sz ora) ->
+          sz = frame_size (fn_frame f) /\ ora = Ptrofs.sub (Ptrofs.repr (align (Z.max 0 sz) 8)) (Ptrofs.repr (size_chunk Mptr));
+
+      wf_allocframe_repr:
+        forall o ff ora,
+          find_instr o (fn_code f) = Some (Pallocframe ff ora) ->
+          align (frame_size ff) 8 - size_chunk Mptr =
+          Ptrofs.unsigned (Ptrofs.sub (Ptrofs.repr (align (frame_size ff) 8)) (Ptrofs.repr (size_chunk Mptr)));
+
+      wf_freeframe_repr:
+        forall o sz ora,
+          find_instr o (fn_code f) = Some (Pfreeframe sz ora) ->
+          Ptrofs.repr (align sz 8 - size_chunk Mptr) = Ptrofs.sub (Ptrofs.repr (align (Z.max 0 sz) 8)) (Ptrofs.repr (size_chunk Mptr));
+      
+    }.
+
+  Definition frame_info_dec (f1 f2: frame_info): { f1 = f2 } + { f1 <> f2 }.
+  Proof.
+    (* frame_perm equality is not decidable... use some encoding based on public/private intervals of offsets in Pallocframe... *)
+  Admitted.
+  
+  Definition is_make_palloc a f :=  a = make_palloc f /\
+                                    align (frame_size f) 8 - size_chunk Mptr =
+                                    Ptrofs.unsigned (Ptrofs.sub (Ptrofs.repr (align (frame_size f) 8)) (Ptrofs.repr (size_chunk Mptr))).
+
+  Definition pallocframe_dec s s' o o': {Pallocframe s o = Pallocframe s' o'} + {Pallocframe s o <> Pallocframe s' o'}.
+  Proof.
+    destruct (frame_info_dec s s'); subst.
+    2: (now right; inversion 1).
+    destruct (Ptrofs.eq_dec o o'); subst.
+    left; reflexivity.
+    right; inversion 1. congruence.
+  Defined.
+
+  Lemma and_dec: forall {A B: Prop},
+      { A } + { ~ A } ->
+      { B } + { ~ B } ->
+      { A /\ B } + { ~ (A /\ B) }.
+  Proof.
+    intros. destruct H, H0; [left|right|right|right]; intuition.
+  Qed.
+
+  Definition is_make_palloc_dec a f : { is_make_palloc a f } + { ~ is_make_palloc a f }.
+  Proof.
+    unfold is_make_palloc, make_palloc.
+    destruct a; try (now right; inversion 1).
+    apply and_dec.
+    apply pallocframe_dec.
+    apply zeq.
+  Defined.
+
+  Definition check_ret_or_jmp roj :=
+    match roj with
+    | Pret | Pjmp _ _ => true
+    | _ => false
+    end.
+
+  Definition valid_ret_or_jmp roj :=
+    match roj with
+    | Pjmp (inl r) _ =>  negb (preg_eq r RSP)
+    | _ => true
+    end.
+  
+  Definition check_free f sz ora :=
+      sz = frame_size (fn_frame f) /\ ora = Ptrofs.sub (Ptrofs.repr (align (Z.max 0 sz) 8)) (Ptrofs.repr (size_chunk Mptr)) /\
+      Ptrofs.repr (align sz 8 - size_chunk Mptr) = Ptrofs.sub (Ptrofs.repr (align (Z.max 0 sz) 8)) (Ptrofs.repr (size_chunk Mptr)).
+
+  Definition check_free_dec f sz ora : { check_free f sz ora } + { ~ check_free f sz ora }.
+  Proof.
+    unfold check_free.
+    apply and_dec. 2: apply and_dec.
+    apply zeq. apply Ptrofs.eq_dec. apply Ptrofs.eq_dec.
+  Defined.
+
+  Definition check_builtin args res :=
+    ~ in_builtin_res res PC /\
+    ~ in_builtin_res res RSP
+    /\ Forall (fun arg : builtin_arg preg => ~ in_builtin_arg arg RA) args.
+
+  Lemma not_in_builtin_res_dec res r:
+    {~ in_builtin_res res r} + {~ ~ in_builtin_res res r}.
+  Proof.
+    induction res; simpl.
+    destruct (preg_eq x r); subst; intuition. left; inversion 1.
+    destruct IHres1, IHres2; try (right; now intuition). left. intuition congruence.
+  Qed.
+
+
+  Lemma not_in_builtin_arg_dec arg r:
+    {~ in_builtin_arg arg r} + {~ ~ in_builtin_arg arg r}.
+  Proof.
+    induction arg; simpl; try (try destr; left; now inversion 1).
+    destruct IHarg1, IHarg2; try (right; now intuition). left. intuition congruence.
+  Qed.
+  
+  Definition check_builtin_dec args res: {check_builtin args res} + { ~ check_builtin args res}.
+  Proof.
+    unfold check_builtin.
+    repeat apply and_dec.
+    apply not_in_builtin_res_dec.
+    apply not_in_builtin_res_dec.
+    apply Forall_dec. intros.
+    apply not_in_builtin_arg_dec.
+  Defined.
+
+  Lemma find_instr_bound:
+    forall c o i,
+      find_instr o c = Some i ->
+      o + instr_size i <= code_size c.
+  Proof.
+    induction c; simpl; intros; eauto. congruence.
+    destr_in H. inv H. generalize (code_size_non_neg c). omega.
+    apply IHc in H. omega.      
+  Qed.
+    
+  Lemma code_bounded_repr':
+    forall c
+      (RNG: 0 <= code_size c <= Ptrofs.max_unsigned)
+      i o
+      (FI: find_instr o c = Some i)
+      sz
+      (LE: 0 <= sz <= instr_size i),
+      Ptrofs.unsigned (Ptrofs.add (Ptrofs.repr o) (Ptrofs.repr sz)) = o + sz.
+  Proof.
+    intros.
+    unfold Ptrofs.add.
+    rewrite (Ptrofs.unsigned_repr sz). 2: generalize (instr_size_repr i); omega.
+    generalize (find_instr_bound _ _ _ FI) (find_instr_pos_positive _ _ _ FI) (instr_size_positive i). intros.
+    rewrite (Ptrofs.unsigned_repr o) by omega.
+    apply Ptrofs.unsigned_repr; omega.
+  Qed.
+
+  Lemma code_bounded_repr:
+    forall c
+      (RNG: 0 <= code_size c <= Ptrofs.max_unsigned)
+      i o
+      (FI: find_instr (Ptrofs.unsigned o) c = Some i)
+      sz
+      (LE: 0 <= sz <= instr_size i),
+      Ptrofs.unsigned (Ptrofs.add o (Ptrofs.repr sz)) = Ptrofs.unsigned o + sz.
+  Proof.
+    intros.
+    erewrite <- code_bounded_repr'; eauto.
+    unfold Ptrofs.add.
+    rewrite Ptrofs.repr_unsigned. reflexivity.
+  Qed.
+
+  Lemma wf_asm_pc_repr' : forall f : function,
+       wf_asm_function f ->
+       forall (i : instruction) (o : ptrofs),
+       find_instr (Ptrofs.unsigned o) (fn_code f) = Some i ->
+       forall sz : Z, 0 <= sz <= instr_size i -> Ptrofs.unsigned (Ptrofs.add o (Ptrofs.repr sz)) = Ptrofs.unsigned o + sz.
+  Proof.
+    intros; eapply code_bounded_repr; eauto.
+    apply wf_asm_code_bounded; eauto.
+  Qed.
+  
+  Fixpoint check_asm_body (f: function) (next_roj: bool) (r: code) : bool :=
+    match r with
+    | nil => negb next_roj
+    | i :: r =>
+      let roj := proj_sumbool (is_free_dec i) in
+      check_asm_body f roj r && 
+      if next_roj then check_ret_or_jmp i && valid_ret_or_jmp i
+      else
+        negb (check_ret_or_jmp i) &&
+        match i with
+        | Pfreeframe sz ora =>     (* after a free, ret or jmp *)
+          check_free_dec f sz ora
+        | Pallocframe _ _ => false (* no alloc in body *)
+        | Pcall (inl r) sg => negb (preg_eq r RSP)
+        | Pbuiltin _ args res => check_builtin_dec args res
+        | _ => true
+      end
+    end.
+  
+  Definition wf_asm_function_check (f: function) : bool :=
+    match fn_code f with
+    | nil => false
+    | a::r => is_make_palloc_dec a (fn_frame f) && check_asm_body f false r
+    end && zle (code_size (fn_code f)) Ptrofs.max_unsigned.
+
+  Lemma check_asm_body_no_alloc:
+    forall f c b i,
+      check_asm_body f b c = true ->
+      In i c ->
+      ~ is_alloc i.
+  Proof.
+    induction c; simpl; intros. easy.
+    intro IA. inv IA.
+    assert (exists b, check_asm_body f b c = true).
+    {
+      eexists. refine (proj1 _); apply andb_true_iff; eauto.
+    }
+    destruct H1.
+    destruct H0. subst. simpl in *.
+    apply andb_true_iff in H. destruct H. destr_in H0.
+    eapply IHc in H0; eauto. apply H0; constructor.
+  Qed.
+  
+  Lemma find_instr_app:
+    forall a o b,
+      0 <= o ->
+      find_instr (o + code_size a) (a ++ b) = find_instr o b.
+  Proof.
+    induction a; simpl; intros; eauto.
+    f_equal. omega.
+    rewrite pred_dec_false.
+    rewrite <- (IHa o b). f_equal. omega. omega.
+    generalize (instr_size_positive a) (code_size_non_neg a0). omega.
+  Qed.
+
+  Lemma find_instr_app':
+    forall a o b,
+      code_size a <= o ->
+      find_instr o (a ++ b) = find_instr (o - code_size a) b.
+  Proof.
+    intros.
+    rewrite <- (find_instr_app a _ b). f_equal. omega. omega.
+  Qed.
+  
+  Lemma find_instr_split:
+    forall c o i,
+      find_instr o c = Some i ->
+      exists a b, c = a ++ i :: b /\ o = code_size a.
+  Proof.
+    induction c; simpl; intros; eauto. congruence.
+    destr_in H. inv H. eexists nil, c; simpl. split; auto.
+    edestruct IHc as (aa & b & EQ & SZ). apply H. subst.
+    exists (a::aa), b; simpl; split; auto. omega.
+  Qed.
+
+  Lemma code_size_app:
+    forall c1 c2,
+      code_size (c1 ++ c2) = code_size c1 + code_size c2.
+  Proof.
+    induction c1; simpl; intros; eauto. rewrite IHc1. omega.
+  Qed.
+  
+  Lemma check_asm_body_after_free:
+    forall f a i b roj,
+      check_asm_body f roj (a ++ i :: b) = true ->
+      is_free i ->
+      check_asm_body f true b = true.
+  Proof.
+    induction a; simpl; intros; eauto.
+    apply andb_true_iff in H. destruct H as (H & _).
+    inv H0. simpl in *. auto.
+    apply andb_true_iff in H. destruct H as (H & B).
+    destruct (is_free_dec a); simpl in *. inv i0.
+    eapply IHa; eauto.
+    eapply IHa; eauto.
+  Qed.
+
+
+  Lemma check_asm_body_call:
+    forall f c b r sg,
+      check_asm_body f b c = true ->
+      In (Pcall (inl r) sg) c ->
+      r <> RSP.
+  Proof.
+    induction c; simpl; intros. easy.
+    assert (exists b, check_asm_body f b c = true).
+    {
+      eexists. refine (proj1 _); apply andb_true_iff; eauto.
+    }
+    apply andb_true_iff in H. destruct H. destruct H1. destruct H0; eauto. subst. simpl in *.
+    destr_in H2; simpl in *. 
+    unfold proj_sumbool in H2; destr_in H2. simpl in H2. congruence.
+  Qed.
+  
+  Lemma check_asm_body_free:
+    forall f c b sz ora,
+      check_asm_body f b c = true ->
+      In (Pfreeframe sz ora) c ->
+      check_free f sz ora.
+  Proof.
+    induction c; simpl; intros. easy.
+    assert (exists b, check_asm_body f b c = true).
+    {
+      eexists. refine (proj1 _); apply andb_true_iff; eauto.
+    }
+    apply andb_true_iff in H. destruct H. destruct H1. destruct H0; eauto. subst. simpl in *.
+    destr_in H2; simpl in *. 
+    unfold proj_sumbool in H2; destr_in H2.
+  Qed.
+ 
+  Lemma check_asm_body_before_roj:
+    forall f a i b roj,
+      check_asm_body f roj (a ++ i :: b) = true ->
+      i = Pret \/ is_jmp i ->
+      (a = nil /\ roj = true) \/ exists a0 i0, a = a0 ++ i0 :: nil /\ is_free i0.
+  Proof.
+    induction a; simpl; intros; eauto.
+    - apply andb_true_iff in H. destruct H as (A & B).
+      destruct H0 as [ROJ|ROJ]; inv ROJ; simpl in *. destr_in B. destr_in B.
+    - apply andb_true_iff in H. destruct H as (A & B).
+      destruct (is_free_dec a); simpl in *. inv i0.
+      + simpl in *. destr_in B. right.
+        destruct a0. clear IHa. simpl in *.
+        eexists nil, _. split. simpl. eauto. constructor.
+        edestruct IHa as [ROJ|(a1 & i1 & EQ & IFR)]; eauto.
+        destruct ROJ; congruence. rewrite EQ.
+        eexists (_ :: a1), i1; split. simpl. reflexivity. auto.
+      + edestruct IHa as [ROJ|(a1 & i1 & EQ & IFR)]; eauto.
+        destruct ROJ; congruence. subst. right.
+        eexists (_ :: a1), i1; split. simpl. reflexivity. auto.
+  Qed.
+
+  Lemma check_asm_body_builtin:
+    forall f c b ef args res,
+      check_asm_body f b c = true ->
+      In (Pbuiltin ef args res) c ->
+      check_builtin args res.
+  Proof.
+    induction c; simpl; intros. easy.
+    assert (exists b, check_asm_body f b c = true).
+    {
+      eexists. refine (proj1 _); apply andb_true_iff; eauto.
+    }
+    destruct H1.
+    destruct H0. subst. simpl in *.
+    apply andb_true_iff in H. destruct H. destr_in H0.
+    unfold proj_sumbool in H0; destr_in H0.
+    eapply IHc in H0; eauto.
+  Qed.
+
+
+  Lemma check_asm_body_jmp:
+    forall f c b r sg,
+      check_asm_body f b c = true ->
+      In (Pjmp (inl r) sg) c ->
+      r <> RSP.
+  Proof.
+    induction c; simpl; intros. easy.
+    assert (exists b, check_asm_body f b c = true).
+    {
+      eexists. refine (proj1 _); apply andb_true_iff; eauto.
+    }
+    apply andb_true_iff in H. destruct H. destruct H1. destruct H0; eauto. subst. simpl in *.
+    destr_in H2; simpl in *. 
+    unfold proj_sumbool in H2; destr_in H2. simpl in H2. congruence.
+  Qed.
+  
+  Lemma wf_asm_function_check_correct f:
+    wf_asm_function_check f = true ->
+    wf_asm_function f.
+  Proof.
+    unfold wf_asm_function_check. destr. simpl. congruence.
+    rewrite ! andb_true_iff. intros ((A & B) & C).
+    unfold proj_sumbool in A, C. destr_in A; destr_in C.
+    clear A C. rename Heqc into CODE. rename l into SIZE.
+    constructor.
+    - rewrite CODE. simpl. intros. destr_in H.
+      apply Asmgenproof0.find_instr_in in H.
+      eapply check_asm_body_no_alloc in H; eauto. contradict H. constructor.
+    - rewrite CODE; simpl. clear - i0. destruct i0 as (A & B). subst. reflexivity.
+    - destruct i0 as (i0 & _). subst. rewrite CODE. simpl.
+      intros. destr_in H. inv H. inv H0.
+      simpl in SIZE.
+      rewrite pred_dec_false.
+      replace (Ptrofs.unsigned (Ptrofs.add o (Ptrofs.repr (instr_size i))) - instr_size (make_palloc (fn_frame f)))
+        with (Ptrofs.unsigned (Ptrofs.add (Ptrofs.repr (Ptrofs.unsigned o - instr_size (make_palloc (fn_frame f)))) (Ptrofs.repr (instr_size i)))).
+      revert H.
+      generalize (Ptrofs.unsigned o - instr_size (make_palloc (fn_frame f))).
+      intros. 
+      edestruct find_instr_split as (a & b & EQ & SZ). apply H. subst.
+      rewrite find_instr_app'.
+      simpl. rewrite pred_dec_false.
+      eapply check_asm_body_after_free in B; eauto.
+      destruct b; simpl in B. congruence. simpl. rewrite pred_dec_true. eexists; split; eauto.
+      apply andb_true_iff in B. destruct B as (B & CHK).
+      unfold check_ret_or_jmp in CHK. apply andb_true_iff in CHK. destruct CHK as (CHK & _). destr_in CHK; try (right; constructor).
+      unfold Ptrofs.add.
+      rewrite (Ptrofs.unsigned_repr (code_size a)).
+      rewrite (Ptrofs.unsigned_repr _ (instr_size_repr i)).
+      rewrite Ptrofs.unsigned_repr. omega.
+      simpl in SIZE. rewrite code_size_app in SIZE. simpl in SIZE.
+      generalize (code_size_non_neg a) (instr_size_positive i) (instr_size_positive i0) (code_size_non_neg b)
+                 (instr_size_positive (make_palloc (fn_frame f))). omega.
+      simpl in SIZE. rewrite code_size_app in SIZE. simpl in SIZE.
+      generalize (code_size_non_neg a) (instr_size_positive i) (instr_size_positive i0) (code_size_non_neg b)
+                 (instr_size_positive (make_palloc (fn_frame f))). omega.
+      unfold Ptrofs.add.
+      rewrite (Ptrofs.unsigned_repr (code_size a)).
+      rewrite (Ptrofs.unsigned_repr _ (instr_size_repr i)).
+      rewrite Ptrofs.unsigned_repr. generalize (instr_size_positive i); omega.
+      simpl in SIZE. rewrite code_size_app in SIZE. simpl in SIZE.
+      generalize (code_size_non_neg a) (instr_size_positive i) (code_size_non_neg b)
+                 (instr_size_positive (make_palloc (fn_frame f))). omega.
+      simpl in SIZE. rewrite code_size_app in SIZE. simpl in SIZE.
+      generalize (code_size_non_neg a) (instr_size_positive i) (code_size_non_neg b)
+                 (instr_size_positive (make_palloc (fn_frame f))). omega.
+      unfold Ptrofs.add.
+      rewrite (Ptrofs.unsigned_repr (code_size a)).
+      rewrite (Ptrofs.unsigned_repr _ (instr_size_repr i)).
+      rewrite Ptrofs.unsigned_repr. generalize (instr_size_positive i); omega.
+      simpl in SIZE. rewrite code_size_app in SIZE. simpl in SIZE.
+      generalize (code_size_non_neg a) (instr_size_positive i) (code_size_non_neg b)
+                 (instr_size_positive (make_palloc (fn_frame f))). omega.
+      simpl in SIZE. rewrite code_size_app in SIZE. simpl in SIZE.
+      generalize (code_size_non_neg a) (instr_size_positive i) (code_size_non_neg b)
+                 (instr_size_positive (make_palloc (fn_frame f))). omega.
+      unfold Ptrofs.add.
+      rewrite (Ptrofs.unsigned_repr _ (instr_size_repr i)).
+      rewrite (Ptrofs.unsigned_repr (Ptrofs.unsigned o - _)).
+      rewrite ! Ptrofs.unsigned_repr. omega.
+      generalize (find_instr_bound _ _ _ H) (find_instr_pos_positive _ _ _ H).
+      generalize (instr_size_positive i)
+                 (instr_size_positive (make_palloc (fn_frame f))). omega.
+      generalize (find_instr_bound _ _ _ H) (find_instr_pos_positive _ _ _ H).
+      generalize (instr_size_positive i)
+                 (instr_size_positive (make_palloc (fn_frame f))). omega.
+      generalize (find_instr_bound _ _ _ H) (find_instr_pos_positive _ _ _ H).
+      generalize (instr_size_positive i)
+                 (instr_size_positive (make_palloc (fn_frame f))). omega.
+      unfold Ptrofs.add.
+      rewrite (Ptrofs.unsigned_repr _ (instr_size_repr i)).
+      rewrite Ptrofs.unsigned_repr.
+      generalize (Ptrofs.unsigned_range o) (instr_size_positive i); omega.
+      generalize (find_instr_bound _ _ _ H) (find_instr_pos_positive _ _ _ H).
+      generalize (instr_size_positive i)
+                 (instr_size_positive (make_palloc (fn_frame f))). omega.
+    - destruct i0 as (i0 & _). subst. rewrite CODE. simpl.
+      intros i o FI ROJ.
+      destr_in FI. inv FI. destruct ROJ as [ROJ|ROJ]; inv ROJ.
+      edestruct find_instr_split as (a & b & EQ & SZ). apply FI. subst.
+      destruct (check_asm_body_before_roj _ _ _ _ _ B ROJ) as [(NIL & ROJFALSE)|(a0 & i0 & EQ & IFR)]. congruence.
+      subst.
+      exists (Ptrofs.sub o (Ptrofs.repr (instr_size i0))), i0.
+      rewrite pred_dec_false.
+      replace (Ptrofs.unsigned (Ptrofs.sub o (Ptrofs.repr (instr_size i0))) - instr_size (make_palloc (fn_frame f))) 
+        with (0 + code_size a0). rewrite app_ass.
+      rewrite find_instr_app. simpl. split; auto. split. auto.
+      unfold Ptrofs.sub. 
+      rewrite (Ptrofs.unsigned_repr _ (instr_size_repr i0)).
+      rewrite Ptrofs.unsigned_repr. omega.
+      generalize (find_instr_bound _ _ _ FI) (find_instr_pos_positive _ _ _ FI). intros.
+      simpl in *. rewrite ! code_size_app in *. simpl in *.
+      generalize (code_size_non_neg a0) (instr_size_positive i) (instr_size_positive i0) (code_size_non_neg b)
+                 (instr_size_positive (make_palloc (fn_frame f))). omega.
+      omega.
+      unfold Ptrofs.sub. 
+      rewrite (Ptrofs.unsigned_repr _ (instr_size_repr i0)).
+      rewrite Ptrofs.unsigned_repr.
+      simpl in *. rewrite ! code_size_app in *. simpl in *. omega.
+      generalize (find_instr_bound _ _ _ FI) (find_instr_pos_positive _ _ _ FI). intros.
+      simpl in *. rewrite ! code_size_app in *. simpl in *.
+      generalize (code_size_non_neg a0) (instr_size_positive i) (instr_size_positive i0) (code_size_non_neg b)
+                 (instr_size_positive (make_palloc (fn_frame f))). omega.
+      unfold Ptrofs.sub. 
+      rewrite (Ptrofs.unsigned_repr _ (instr_size_repr i0)).
+      rewrite Ptrofs.unsigned_repr.
+      simpl in *. rewrite ! code_size_app in *. simpl in *.
+      generalize (find_instr_bound _ _ _ FI) (find_instr_pos_positive _ _ _ FI). intros. 
+      simpl in *. rewrite ! code_size_app in *. simpl in *.
+      generalize (code_size_non_neg a0) (instr_size_positive i) (instr_size_positive i0) (code_size_non_neg b)
+                 (instr_size_positive (make_palloc (fn_frame f))). omega.
+      generalize (find_instr_bound _ _ _ FI) (find_instr_pos_positive _ _ _ FI). intros. 
+      simpl in *. rewrite ! code_size_app in *. simpl in *.
+      generalize (code_size_non_neg a0) (instr_size_positive i) (instr_size_positive i0) (code_size_non_neg b)
+                 (instr_size_positive (make_palloc (fn_frame f))). omega.
+    - rewrite CODE; split; auto.
+      generalize (code_size_non_neg (i::c)). omega.
+    - destruct i0 as (i0 & _). subst. rewrite CODE. simpl.
+      intros o ef args res FI.
+      destr_in FI. inv FI.
+      apply Asmgenproof0.find_instr_in in FI.
+      eapply check_asm_body_builtin in FI; eauto.
+    - destruct i0 as (i0 & _). subst. rewrite CODE. simpl.
+      intros o r sg FI.
+      destr_in FI. inv FI.
+      apply Asmgenproof0.find_instr_in in FI.
+      eapply check_asm_body_jmp in FI; eauto.
+    - destruct i0 as (i0 & _). subst. rewrite CODE. simpl.
+      intros o r sg FI.
+      destr_in FI. inv FI.
+      apply Asmgenproof0.find_instr_in in FI.
+      eapply check_asm_body_call in FI; eauto.
+    - destruct i0 as (i0 & _). subst. rewrite CODE. simpl.
+      intros o sz ora FI.
+      destr_in FI. inv FI.
+      apply Asmgenproof0.find_instr_in in FI.
+      edestruct check_asm_body_free as (A & BB & C); subst; eauto.
+    - destruct i0 as (i0 & PA). subst. rewrite CODE. simpl.
+      intros o ff ora FI.
+      destr_in FI. inv FI; auto.
+      apply Asmgenproof0.find_instr_in in FI.
+      eapply check_asm_body_no_alloc in FI; eauto. contradict FI; constructor.
+    - destruct i0 as (i0 & _). subst. rewrite CODE. simpl.
+      intros o sz ora FI.
+      destr_in FI. inv FI.
+      apply Asmgenproof0.find_instr_in in FI.
+      edestruct check_asm_body_free as (A & BB & C); subst; eauto.
+  Qed.
+
+  Lemma wf_asm_pc_repr:
+    forall f (WF: wf_asm_function f) i o,
+      find_instr (Ptrofs.unsigned o) (fn_code f) = Some i ->
+      Ptrofs.unsigned (Ptrofs.add o (Ptrofs.repr (instr_size i))) = Ptrofs.unsigned o + instr_size i.
+  Proof.
+    intros; eapply wf_asm_pc_repr'; eauto. generalize (instr_size_positive i); omega.
+  Qed.
+
+  Lemma wf_asm_wf_allocframe:
+    forall f (WF: wf_asm_function f) o fi ora
+      (FI: find_instr o (fn_code f) = Some (Pallocframe fi ora)),
+      make_palloc (fn_frame f) = Pallocframe fi ora.
+  Proof.
+    intros.
+    exploit wf_asm_alloc_only_at_beginning; eauto. intro; subst.
+    erewrite wf_asm_alloc_at_beginning in FI; eauto. inv FI; auto.
+  Qed.
+
+End WFASM.
 
 Section WITHMEMORYMODEL.
 
@@ -37,22 +647,14 @@ Section WITHGE.
     | Pload_parent_pointer rd z =>
       let sp := Val.offset_ptr (rs RSP) (Ptrofs.repr (align (Z.max 0 z) 8)) in
       Next (nextinstr (rs#rd <- sp) sz) m
-    | Pcall_s id sg =>
+    | Pcall ros sg =>
+      let addr := eval_ros ge ros rs in
       let sp := Val.offset_ptr (rs RSP) (Ptrofs.neg (Ptrofs.repr (size_chunk Mptr))) in
       match Mem.storev Mptr m sp (Val.offset_ptr rs#PC sz) with
       | None => Stuck
       | Some m2 =>
         Next (rs#RA <- (Val.offset_ptr rs#PC sz)
-                #PC <- (Genv.symbol_address ge id Ptrofs.zero)
-                #RSP <- sp) m2
-      end
-    | Pcall_r r sg =>
-      let sp := Val.offset_ptr (rs RSP) (Ptrofs.neg (Ptrofs.repr (size_chunk Mptr))) in
-      match Mem.storev Mptr m sp (Val.offset_ptr rs#PC sz) with
-      | None => Stuck
-      | Some m2 =>
-        Next (rs#RA <- (Val.offset_ptr rs#PC sz)
-                #PC <- (rs r)
+                #PC <- addr
                 #RSP <- sp) m2
       end
     | Pret =>
@@ -110,14 +712,15 @@ End WITHGE.
 
   Inductive initial_state_gen (prog: Asm.program) (rs: regset) m: state -> Prop :=
   | initial_state_gen_intro:
-      forall m1 bstack m2 m3 m4
+      forall m1 bstack m2 m3 m4 bmain
         (MALLOC: Mem.alloc (Mem.push_new_stage m) 0 (Mem.stack_limit + align (size_chunk Mptr) 8) = (m1,bstack))
         (MDROP: Mem.drop_perm m1 bstack 0 (Mem.stack_limit + align (size_chunk Mptr) 8) Writable = Some m2)
         (MRSB: Mem.record_stack_blocks m2 (make_singleton_frame_adt' bstack frame_info_mono 0) = Some m3)
         (STORE_RETADDR: Mem.storev Mptr m3 (Vptr bstack (Ptrofs.repr (Mem.stack_limit + align (size_chunk Mptr) 8 - size_chunk Mptr))) Vnullptr = Some m4),
         let ge := Genv.globalenv prog in
+        Genv.find_symbol ge prog.(prog_main) = Some bmain ->
         let rs0 :=
-            rs # PC <- (Genv.symbol_address ge prog.(prog_main) Ptrofs.zero)
+            rs #PC <- (Vptr bmain Ptrofs.zero)
                #RA <- Vnullptr
                #RSP <- (Val.offset_ptr (Vptr bstack (Ptrofs.repr (Mem.stack_limit + align (size_chunk Mptr) 8))) (Ptrofs.neg (Ptrofs.repr (size_chunk Mptr)))) in
         initial_state_gen prog rs m (State rs0 m4).
@@ -134,4 +737,340 @@ End WITHGE.
   Definition semantics prog rs :=
     Semantics step (initial_state prog rs) final_state (Genv.globalenv prog).
 
+  Definition rs_state s :=
+    let '(State rs _) := s in rs.
+  Definition m_state s :=
+    let '(State _ m) := s in m.
+
+  Section INVARIANT.
+    Context {memory_model: @Mem.MemoryModel mem memory_model_ops }.
+    Existing Instance inject_perm_upto_writable.
+    Existing Instance symbols_inject_instance.
+    Context `{external_calls_props : !ExternalCallsProps mem
+                                      (memory_model_ops := memory_model_ops)
+             }.
+    Variable prog: Asm.program.
+    Let ge := Genv.globalenv prog.
+    Definition bstack := Genv.genv_next ge.
+
+    Definition rsp_ptr (s: state) : Prop :=
+      exists o, rs_state s RSP = Vptr bstack o /\ (align_chunk Mptr | Ptrofs.unsigned o).
+
+    Definition bstack_perm (s: state) : Prop :=
+      forall o k p,
+        Mem.perm (m_state s) bstack o k p ->
+        Mem.perm (m_state s) bstack o k Writable.
+
+    Definition stack_top_state (s: state) : Prop :=
+      is_stack_top (Mem.stack (m_state s)) bstack.
+
+    Inductive real_asm_inv : state -> Prop := 
+    | real_asm_inv_intro:
+        forall s
+          (RSPPTR: rsp_ptr s)
+          (BSTACKPERM: bstack_perm s)
+          (STOP: stack_top_state s),
+          real_asm_inv s.
+
+    Lemma real_initial_inv:
+      forall rs0 is,
+        initial_state prog rs0 is -> real_asm_inv is.
+    Proof.
+      intros rs0 is IS; inv IS. inv H0.
+      constructor.
+      - red. simpl; unfold rs1; simpl_regs; simpl.
+        exploit Mem.alloc_result; eauto. rewnb.
+        fold ge. intro; subst.
+        eexists; split; eauto.
+        apply div_ptr_add.
+        apply div_unsigned_repr.
+        apply Z.divide_add_r. apply align_Mptr_stack_limit. apply align_Mptr_align8.
+        apply align_Mptr_modulus. unfold Ptrofs.neg. apply div_unsigned_repr.
+        apply Zdivide_opp_r.
+        apply div_unsigned_repr.
+        apply align_size_chunk_divides.
+        apply align_Mptr_modulus.
+        apply align_Mptr_modulus.
+        apply align_Mptr_modulus.
+      - exploit Mem.alloc_result; eauto. rewnb.
+        fold ge. intro; subst.
+        red. simpl. intros o k p. repeat rewrite_perms. unfold bstack. rewrite ! pred_dec_true by reflexivity.
+        intros (A & B); split; auto. constructor.
+      - red. simpl. repeat rewrite_stack_blocks.
+        intros A. inv A. red; simpl. left.
+        exploit Mem.alloc_result; eauto. rewnb.
+        fold ge. unfold bstack. auto.
+    Qed.
+
+    Lemma exec_instr_invar_same:
+      forall f i rs1 m1,
+        stack_invar i = true ->
+        exec_instr ge f i rs1 m1 = RawAsm.exec_instr ge f i rs1 m1.
+    Proof.
+      intros f i rs1 m1 SI.
+      destruct i; simpl in SI; simpl; congruence.
+    Qed.
+
+    Inductive is_load_parent_pointer: instruction -> Prop :=
+    | ilpp_intro i z: is_load_parent_pointer (Pload_parent_pointer i z).
+
+    Lemma is_load_parent_pointer_dec i: { is_load_parent_pointer i } + { ~ is_load_parent_pointer i }.
+    Proof.
+      destruct i; first [ now (right; inversion 1) | left; econstructor ].
+    Defined.
+
+    Lemma exec_instr_invar_same':
+      forall f i rs1 m1 l,
+        stack_invar i = true ->
+        ~ is_load_parent_pointer i ->
+        Asm.exec_instr l ge f i rs1 m1 = RawAsm.exec_instr ge f i rs1 m1.
+    Proof.
+      intros f i rs1 m1 l SI NILPP.
+      destruct i; simpl in SI; simpl; try congruence.
+      contradict NILPP. constructor.
+    Qed.
+
+    Lemma exec_instr_invar_inv:
+      forall f i rs1 m1 rs2 m2,
+        asm_instr_no_rsp i ->
+        stack_invar i = true ->
+        exec_instr ge f i rs1 m1 = Next rs2 m2 ->
+        real_asm_inv (State rs1 m1) ->
+        real_asm_inv (State rs2 m2).
+    Proof.
+      intros f i rs1 m1 rs2 m2 NORSP INVAR EI RAI; inv RAI.
+      destruct (is_load_parent_pointer_dec i).
+      - constructor.
+        + red in RSPPTR; red.
+          simpl in *.
+          destruct RSPPTR as (o & EQ & AL).
+          red in NORSP.
+          inv i0. simpl in EI. inv EI.
+          simpl_regs.
+          setoid_rewrite Pregmap.gsspec. destr. inv e. rewrite EQ.
+          simpl.
+          eexists; split; eauto. apply div_ptr_add. auto. apply div_unsigned_repr.
+          transitivity 8.
+          unfold Mptr. destr; simpl. exists 1; omega. exists 2; omega.
+          apply align_divides. omega.
+          apply align_Mptr_modulus.
+          apply align_Mptr_modulus.
+          eauto.
+        + red in BSTACKPERM; red. simpl in *. intros.
+          inv i0; simpl in EI; inv EI. eauto.
+        + red in STOP; red. simpl in *.
+          inv i0; simpl in EI; inv EI. eauto.
+      - erewrite exec_instr_invar_same in EI; eauto.
+        erewrite <- exec_instr_invar_same' with (l:=nil) in EI; eauto.
+        exploit NORSP; eauto. intro EQ.
+        generalize (asmgen_no_change_stack i INVAR _ _ _ _ _ _ _ EI). intros (A & B).
+        constructor.
+        + red in RSPPTR; red. simpl in *; rewrite EQ. eauto.
+        + red in BSTACKPERM; red. simpl in *. setoid_rewrite B. eauto.
+        + red in STOP; red; simpl in *. rewrite A; eauto.
+    Qed.
+
+    Lemma align_Mptr_sub:
+      forall o,
+        (align_chunk Mptr | Ptrofs.unsigned o) ->
+        (align_chunk Mptr | Ptrofs.unsigned (Ptrofs.add o (Ptrofs.neg (Ptrofs.repr (size_chunk Mptr))))).
+    Proof.
+      intros.
+      apply div_ptr_add; auto.
+      apply div_unsigned_repr.
+      apply Z.divide_opp_r.
+      apply div_unsigned_repr.
+      apply align_size_chunk_divides.
+      apply align_Mptr_modulus.
+      apply align_Mptr_modulus.
+      apply align_Mptr_modulus.
+    Qed.
+
+    Lemma align_Mptr_add:
+      forall o,
+        (align_chunk Mptr | Ptrofs.unsigned o) ->
+        (align_chunk Mptr | Ptrofs.unsigned (Ptrofs.add o (Ptrofs.repr (size_chunk Mptr)))).
+    Proof.
+      intros.
+      apply div_ptr_add; auto.
+      apply div_unsigned_repr.
+      apply align_size_chunk_divides.
+      apply align_Mptr_modulus.
+      apply align_Mptr_modulus.
+    Qed.
+
+    Lemma align_Mptr_add_gen:
+      forall o d,
+        (align_chunk Mptr | Ptrofs.unsigned o) ->
+        (align_chunk Mptr | Ptrofs.unsigned d) ->
+        (align_chunk Mptr | Ptrofs.unsigned (Ptrofs.add o d)).
+    Proof.
+      intros.
+      apply div_ptr_add; auto.
+      apply align_Mptr_modulus.
+    Qed.
+
+    Definition asm_prog_no_rsp (ge: Genv.t Asm.fundef unit):=
+      forall b f,
+        Genv.find_funct_ptr ge b = Some (Internal f) ->
+        asm_code_no_rsp (fn_code f).
+
+    Definition wf_asm_prog (ge: Genv.t Asm.fundef unit):=
+      forall b f,
+        Genv.find_funct_ptr ge b = Some (Internal f) ->
+        wf_asm_function f.
+    
+    Lemma real_asm_inv_inv:
+      forall (prog_no_rsp: asm_prog_no_rsp ge) (WF: wf_asm_prog ge) s1 t s2,
+        step ge s1 t s2 ->
+        real_asm_inv s1 ->
+        real_asm_inv s2.
+    Proof.
+      intros prog_no_rsp WF s1 t s2 STEP INV; inv STEP.
+      - destruct (stack_invar i) eqn:INVAR.
+        eapply exec_instr_invar_inv; eauto.
+        eapply prog_no_rsp; eauto. eapply Asmgenproof0.find_instr_in; eauto.
+        destruct i; simpl in INVAR; try congruence.
+        + (* call_s *)
+          simpl in H2. destr_in H2. inv H2. inv INV; constructor; simpl.
+          * red. simpl. simpl_regs. destruct RSPPTR as (o & EQ & AL); simpl in *; rewrite EQ.
+            simpl. eexists; split; eauto. apply align_Mptr_sub; auto.
+          * red in BSTACKPERM; red; simpl in *.
+            intros o k p. repeat rewrite_perms; eauto.
+          * red in STOP; red; simpl in *. repeat rewrite_stack_blocks; eauto.
+        + (* ret *)
+          simpl in H2; repeat destr_in H2; inv INV; constructor; simpl.
+          * red. simpl. simpl_regs. destruct RSPPTR as (o & EQ & AL); simpl in *; rewrite EQ.
+            simpl. eexists; split; eauto. apply align_Mptr_add; auto.
+          * red in BSTACKPERM; red; simpl in *.
+            intros o k p. repeat rewrite_perms; eauto.
+          * red in STOP; red; simpl in *. repeat rewrite_stack_blocks; eauto.
+        + (* allocframe *)
+          simpl in H2; repeat destr_in H2; inv INV; constructor; simpl.
+          * red. simpl. simpl_regs. destruct RSPPTR as (o & EQ & AL); simpl in *; rewrite EQ.
+            simpl. eexists; split; eauto. apply align_Mptr_add_gen; auto.
+            unfold Ptrofs.neg. apply div_unsigned_repr; auto. apply Z.divide_opp_r.
+            unfold Ptrofs.sub. apply div_unsigned_repr; auto.
+            apply Z.divide_sub_r.
+            apply div_unsigned_repr; auto.
+            transitivity 8. unfold Mptr. destr; simpl. exists 1; omega. exists 2; omega. apply align_divides. omega.
+            apply align_Mptr_modulus.
+            apply div_unsigned_repr; auto.
+            apply align_size_chunk_divides.
+            apply align_Mptr_modulus.
+            apply align_Mptr_modulus.
+            apply align_Mptr_modulus.
+          * red in BSTACKPERM; red; simpl in *.
+            intros o k p. repeat rewrite_perms; eauto.
+          * red in STOP; red; simpl in *. repeat rewrite_stack_blocks; eauto.
+        + (* freeframe *)
+          simpl in H2; repeat destr_in H2; inv INV; constructor; simpl.
+          * red. simpl. simpl_regs. destruct RSPPTR as (o & EQ & AL); simpl in *; rewrite EQ.
+            simpl. eexists; split; eauto. apply align_Mptr_add_gen; auto.
+            unfold Ptrofs.sub. apply div_unsigned_repr; auto.
+            apply Z.divide_sub_r.
+            apply div_unsigned_repr; auto.
+            transitivity 8. unfold Mptr. destr; simpl. exists 1; omega. exists 2; omega. apply align_divides. omega.
+            apply align_Mptr_modulus.
+            apply div_unsigned_repr; auto.
+            apply align_size_chunk_divides.
+            apply align_Mptr_modulus.
+            apply align_Mptr_modulus.
+          * red in BSTACKPERM; red; simpl in *.
+            intros o k p. repeat rewrite_perms; eauto.
+          * red in STOP; red; simpl in *. repeat rewrite_stack_blocks; eauto.
+      - inv INV; constructor.
+        + red in RSPPTR; red; simpl in *. unfold nextinstr_nf. repeat simpl_regs.
+          rewrite Asmgenproof0.undef_regs_other.
+          2: simpl; intuition subst; congruence.
+          exploit wf_asm_builtin_not_PC; eauto.
+          intros (NPC & NRSP & NRA).
+          rewrite set_res_other; auto.
+          rewrite Asmgenproof0.undef_regs_other.
+          eauto. setoid_rewrite in_map_iff. intros r' (x & PREG & IN). subst.
+          intro EQ. symmetry in EQ. apply preg_of_not_rsp in EQ. congruence.
+        + red in BSTACKPERM; red. simpl in *. intros o k p.
+          repeat rewrite_perms. eauto.
+          red in STOP; simpl in STOP. eapply is_stack_top_in_stack; eauto.
+          red in STOP; simpl in STOP. eapply is_stack_top_in_stack; eauto.
+        + red in STOP; red; simpl in *. rewrite_stack_blocks. auto.
+      - inv INV; constructor.
+        + Opaque destroyed_at_call.
+          red in RSPPTR; red; simpl in *. repeat simpl_regs.
+          destruct RSPPTR as (o & EQ & AL); simpl in *; rewrite EQ.
+          simpl. eexists; split; eauto. apply align_Mptr_add; auto.
+        + red in BSTACKPERM; red. simpl in *. intros o k p.
+          repeat rewrite_perms. eauto.
+          red in STOP; simpl in STOP. eapply is_stack_top_in_stack; eauto.
+          red in STOP; simpl in STOP. eapply is_stack_top_in_stack; eauto.
+        + red in STOP; red; simpl in *. rewrite_stack_blocks. auto.        
+    Qed.
+
+End INVARIANT.
+
 End WITHMEMORYMODEL.
+
+Section RECEPTIVEDET.
+
+  Context `{memory_model: Mem.MemoryModel }.
+  Existing Instance inject_perm_upto_writable.
+
+  Context `{external_calls_ops : !ExternalCallsOps mem }.
+  Context `{!EnableBuiltins mem}.
+
+  Existing Instance mem_accessors_default.
+  Existing Instance symbols_inject_instance.
+  Context `{external_calls_props : !ExternalCallsProps mem
+                                    (memory_model_ops := memory_model_ops)
+           }.
+
+  Theorem real_asm_single_events p rs:
+    single_events (semantics p rs).
+  Proof.
+    red. simpl. intros s t s' STEP.
+    inv STEP; simpl. omega.
+    eapply external_call_trace_length; eauto.
+    eapply external_call_trace_length; eauto.
+  Qed.
+
+  Theorem real_asm_receptive p rs:
+    receptive (semantics p rs).
+  Proof.
+    split.
+    - simpl. intros s t1 s1 t2 STEP MT.
+      inv STEP.
+      inv MT. eexists. eapply exec_step_internal; eauto.
+      edestruct external_call_receptive as (vres2 & m2 & EC2); eauto.
+      eexists. eapply exec_step_builtin; eauto.
+      edestruct external_call_receptive as (vres2 & m2 & EC2); eauto.
+      eexists. eapply exec_step_external; eauto.
+    - eapply real_asm_single_events; eauto.
+  Qed.
+
+  Theorem real_asm_determinate p rs:
+    determinate (semantics p rs).
+  Proof.
+    split.
+    - simpl; intros s t1 s1 t2 s2 STEP1 STEP2.
+      inv STEP1.
+      + inv STEP2; rewrite_hyps. split. constructor.  congruence.
+        simpl in H2. inv H2.
+      + inv STEP2; rewrite_hyps. inv H11.
+        exploit eval_builtin_args_determ. apply H2. apply H9. intro; subst.
+        exploit external_call_determ. apply H3. apply H10. intros (A & B); split; auto. intro C.
+        destruct B; auto. congruence.
+      + inv STEP2; rewrite_hyps.
+        exploit extcall_arguments_determ. apply H1. apply H7. intro; subst.
+        exploit external_call_determ. apply H2. apply H8. intros (A & B); split; auto. intro C.
+        destruct B; auto. congruence.
+    - apply real_asm_single_events.
+    - simpl. intros s1 s2 IS1 IS2; inv IS1; inv IS2. rewrite_hyps.
+      inv H0; inv H2. rewrite_hyps. unfold rs0, rs1, ge, ge0 in *. rewrite_hyps. congruence.
+    - simpl. intros s r FS.
+      red. intros t s' STEP.
+      inv FS. inv STEP; rewrite_hyps.
+    - simpl. intros s r1 r2 FS1 FS2.
+      inv FS1; inv FS2. congruence.
+  Qed.
+
+End RECEPTIVEDET.
