x86/Asmgenproof.v
@@ -719,270 +719,6 @@ Proof.
     simpl. rewrite BLOCKS. eauto.
 Qed.
 
-Lemma mk_setcc_app:
-  forall cond x c,
-    mk_setcc cond x c = mk_setcc cond x nil ++ c.
-Proof.
-  unfold mk_setcc, mk_setcc_base.
-  intros. repeat destr.
-Qed.
-
-Lemma transl_cond_app:
-  forall a b cond lr tc,
-    transl_cond cond lr (a ++ b) = OK tc ->
-    exists tc', transl_cond cond lr a = OK tc' /\ tc = tc' ++ b.
-Proof.
-  intros a b cond lr tc TC.
-  unfold transl_cond in *.
-  repeat destr_in TC; monadInv H0; rewrite EQ, ? EQ1; simpl; eauto.
-Qed.
-
-Lemma transl_op_eq:
-  forall op lr r c tc,
-    transl_op op lr r c = OK tc ->
-    exists ti,
-      transl_op op lr r nil = OK ti /\ tc = ti ++ c.
-Proof.
-  intros op lr r c tc TO.
-  destruct op; simpl in *; repeat destr_in TO; eauto; try (monadInv H0; rewrite EQ; simpl; now eauto).
-  - unfold mk_mov in *. repeat destr_in H0; eauto.
-  - monadInv H0. rewrite EQ, EQ1. simpl.
-    unfold mk_intconv in *. repeat destr_in EQ2; eauto.
-  - monadInv H0. rewrite EQ, EQ1. simpl.
-    unfold mk_intconv in *. repeat destr_in EQ2; eauto.
-  - monadInv H0. rewrite EQ, EQ1. simpl.
-    unfold mk_intconv in *. repeat destr_in EQ2; eauto.
-  - monadInv H0. rewrite EQ, EQ1. simpl.
-    unfold mk_intconv in *. repeat destr_in EQ2; eauto.
-  - monadInv H0. rewrite EQ, EQ1. simpl.
-    unfold mk_intconv in *. repeat destr_in EQ2; eauto.
-  - monadInv H0. rewrite EQ, EQ1. simpl.
-    unfold mk_intconv in *. repeat destr_in EQ2; eauto.
-  - monadInv H0. rewrite EQ, EQ1. simpl.
-    unfold mk_intconv in *. repeat destr_in EQ2; eauto.
-  - monadInv H0. rewrite EQ, EQ1. simpl.
-    unfold mk_intconv in *. repeat destr_in EQ2; eauto.
-  - monadInv H0. rewrite EQ, EQ1. simpl.
-    unfold mk_intconv in *. repeat destr_in EQ2; eauto.
-  - unfold mk_shrximm.  eauto.
-  - monadInv H0. rewrite EQ, EQ1. simpl. eauto.
-  - monadInv H0. rewrite EQ, EQ1. simpl. eauto.
-  - monadInv H0. rewrite EQ, EQ1. simpl. eauto.
-  - monadInv H0. rewrite EQ, EQ1. simpl. eauto.
-  - monadInv H0. rewrite EQ, EQ1. simpl. eauto.
-  - monadInv H0. rewrite EQ, EQ1. simpl. eauto.
-  - monadInv H0. rewrite EQ, EQ1. simpl. eauto.
-  - monadInv H0. rewrite EQ, EQ1. simpl. eauto.
-  - monadInv H0. rewrite EQ, EQ1. simpl. eauto.
-  - unfold mk_shrxlimm. destr. eauto. eauto.
-  - monadInv H0. rewrite EQ, EQ1. simpl. repeat destr; eauto.
-  - monadInv H0. rewrite EQ, EQ1. simpl. eauto.
-  - monadInv H0. rewrite EQ, EQ1. simpl. eauto.
-  - monadInv H0. rewrite EQ, EQ1. simpl. eauto.
-  - monadInv H0. rewrite EQ, EQ1. simpl. eauto.
-  - monadInv H0. rewrite EQ, EQ1. simpl. eauto.
-  - monadInv H0. rewrite EQ, EQ1. simpl. eauto.
-  - monadInv H0. rewrite EQ, EQ1. simpl. eauto.
-  - monadInv H0. rewrite EQ, EQ1. simpl. eauto.
-  - monadInv H0. rewrite EQ, EQ1. simpl. eauto.
-  - monadInv H0. rewrite EQ, EQ1. simpl. eauto.
-  - monadInv H0. rewrite EQ, EQ1. simpl. eauto.
-  - monadInv H0. rewrite EQ, EQ1. simpl. eauto.
-  - monadInv H0. rewrite EQ, EQ1. simpl. eauto.
-  - monadInv H0. rewrite EQ, EQ1. simpl. eauto.
-  - monadInv H0. rewrite EQ, EQ1. simpl. eauto.
-  - monadInv H0. rewrite EQ, EQ1. simpl. eauto.
-  - monadInv H0. rewrite EQ, EQ1. simpl. eauto.
-  - monadInv H0. rewrite EQ, EQ1. simpl. eauto.
-  - monadInv H0. rewrite EQ.
-    rewrite mk_setcc_app in EQ0.
-    edestruct transl_cond_app as (tc' & TC & APP); eauto.
-Qed.
-
-Lemma transl_cond_app':
-  forall a b cond lr tc,
-    transl_cond cond lr a = OK tc ->
-    transl_cond cond lr (a ++ b) = OK (tc ++ b).
-Proof.
-  intros a b cond lr tc TC.
-  unfold transl_cond in *.
-  repeat destr_in TC; monadInv H0; rewrite EQ, ? EQ1; simpl; eauto.
-Qed.
-
-Lemma mk_setcc_app':
-  forall cond x c c',
-    mk_setcc cond x (c ++ c') = mk_setcc cond x c ++ c'.
-Proof.
-  unfold mk_setcc, mk_setcc_base.
-  intros. repeat destr.
-Qed.
-
-Lemma transl_op_eq':
-  forall op lr r c c' tc,
-    transl_op op lr r c = OK tc ->
-    transl_op op lr r (c ++ c') = OK (tc ++ c').
-Proof.
-  intros op lr r c c' tc TO;
-    destruct op; simpl in *;
-      repeat match goal with
-             | H: bind _ _ = _ |- _ => monadInv H
-             | H: ?a = OK ?b |- context [bind ?a _] => rewrite H; simpl; eauto
-             | H: mk_mov _ _ _ = _ |- _ => unfold mk_mov in H; repeat destr_in H
-             | H: mk_intconv _ _ _ _ = _ |- _ => unfold mk_intconv in H; inv H; eauto
-             | H: context [match ?a with _ => _ end] |- _ => repeat destr_in H
-             | H: OK _ = OK _ |- _ => inv H
-             | H: Error _ = OK _ |- _ => inv H
-             | |- _ => simpl in *; eauto
-             end.
-  unfold mk_shrxlimm. destr; eauto.
-  repeat destr; eauto.
-  rewrite mk_setcc_app'.
-  eapply transl_cond_app'; eauto.
-Qed.    
-
-Lemma transl_load_eq:
-  forall m a l m0 c tc
-    (TI : transl_load m a l m0 c = OK tc),
-  exists ti, transl_load m a l m0 nil = OK ti /\ tc = ti ++ c.
-Proof.
-  intros.
-  unfold transl_load. monadInv TI. monadInv EQ. repeat destr_in EQ1; rewrite EQ0; simpl; rewrite H0; simpl; eauto.
-Qed.
-
-Lemma mk_storebyte_eq:
-  forall x x0 c tc
-    (EQ1 : mk_storebyte x x0 c = OK tc),
-  exists ti, mk_storebyte x x0 nil = OK ti /\ tc = ti ++ c.
-Proof.
-  unfold mk_storebyte.
-  intros. inv EQ1. eauto.
-Qed.
-
-
-Lemma transl_store_eq:
-  forall m a l m0 c tc
-    (TI : transl_store m a l m0 c = OK tc),
-  exists ti, transl_store m a l m0 nil = OK ti /\ tc = ti ++ c.
-Proof.
-  intros.
-  unfold transl_store. monadInv TI. rewrite EQ; simpl.
-  repeat destr_in EQ0; monadInv H0; rewrite EQ0; simpl; eauto using mk_storebyte_eq.
-Qed.
-
-
-Lemma transl_load_eq':
-  forall m a l m0 c c' tc
-    (TI : transl_load m a l m0 c = OK tc),
-    transl_load m a l m0 (c ++ c') = OK (tc ++ c').
-Proof.
-  intros.
-  unfold transl_load. monadInv TI. monadInv EQ. rewrite EQ0. simpl.
-  repeat destr_in EQ1; simpl; rewrite H0; simpl; eauto.
-Qed.
-
-Lemma mk_storebyte_eq':
-  forall x x0 c c' tc
-    (EQ1 : mk_storebyte x x0 c = OK tc),
-    mk_storebyte x x0 (c ++ c') = OK (tc ++ c').
-Proof.
-  unfold mk_storebyte.
-  intros. inv EQ1. eauto.
-Qed.
-
-Lemma transl_store_eq':
-  forall m a l m0 c c' tc
-    (TI : transl_store m a l m0 c = OK tc),
-    transl_store m a l m0 (c ++ c') = OK (tc ++ c').
-Proof.
-  intros.
-  unfold transl_store. monadInv TI. rewrite EQ; simpl.
-  repeat destr_in EQ0; monadInv H0; rewrite EQ0; simpl; eauto using mk_storebyte_eq'.
-Qed.
-
-
-Lemma mk_jcc_app:
-  forall cond x c,
-    mk_jcc cond x c = mk_jcc cond x nil ++ c.
-Proof.
-  unfold mk_jcc.
-  intros. repeat destr.
-Qed.
-
-Lemma transl_instr_eq:
-  forall f i ax c tc,
-    transl_instr f i ax c = OK tc ->
-    exists ti,
-      transl_instr f i ax nil = OK ti /\ tc = ti ++ c.
-Proof.
-  intros f i ax c tc TI.
-  destruct i; simpl in *.
-  - Transparent loadind.
-    monadInv TI. unfold loadind. repeat destr_in EQ; simpl; eauto.
-  - monadInv TI. unfold storeind. repeat destr_in EQ; simpl; eauto.
-  - destr.
-    monadInv TI. unfold loadind. repeat destr_in EQ; simpl; eauto.
-    monadInv TI. monadInv EQ. unfold loadind. repeat destr_in EQ0; simpl; eauto.
-  - edestruct transl_op_eq as (ti & TOP & EQ); eauto.
-  - eauto using transl_load_eq.
-  - eauto using transl_store_eq.
-  - destr_in TI; monadInv TI; rewrite ? EQ; simpl; eauto.
-  - destr_in TI; monadInv TI; rewrite ? EQ; simpl; eauto.
-  - inv TI; eauto.
-  - inv TI; eauto.
-  - inv TI; eauto.
-  - eapply transl_cond_app; eauto. erewrite <- mk_jcc_app. auto.
-  - monadInv TI; rewrite EQ; simpl; eauto.
-  - inv TI. eauto.
-Qed.
-
-Lemma mk_jcc_app':
-  forall cond x c c',
-    mk_jcc cond x (c ++ c') = mk_jcc cond x c ++ c'.
-Proof.
-  unfold mk_jcc.
-  intros. repeat destr.
-Qed.
-
-Lemma transl_instr_eq':
-  forall f i ax c c' tc,
-    transl_instr f i ax c = OK tc ->
-    transl_instr f i ax (c ++ c') = OK (tc ++ c').
-Proof.
-  intros f i ax c c' tc TI.
-  destruct i; simpl in *; repeat destr_in TI;
-    repeat match goal with
-           | H: loadind _ _ _ _ _ = _ |- _ => unfold loadind in *; monadInv H
-           | H: storeind _ _ _ _ _ = _ |- _ => unfold storeind in *; monadInv H
-           | H: bind _ _ = _ |- _ => monadInv H
-           | H: ?a = OK ?b |- context [bind ?a _] => rewrite H; simpl; eauto
-           | H: context [match ?a with _ => _ end] |- _ => repeat destr_in H
-           | H: OK _ = OK _ |- _ => inv H
-           | |- _ => simpl in *; eauto
-           end.
-  eapply transl_op_eq'; eauto.
-  eapply transl_load_eq'; eauto.
-  eapply transl_store_eq'; eauto.
-  rewrite mk_jcc_app'. eapply transl_cond_app'; eauto.
-Qed.
-
-Lemma transl_code_app:
-  forall f l1 l2 ep1 x,
-    transl_code f (l1 ++ l2) ep1 = OK x ->
-    exists ep2 y, transl_code f l1 ep1 = OK y /\ bind (transl_code f l2 ep2) (fun k => OK (y ++ k)) = OK x.
-Proof.
-  induction l1; simpl; intros; eauto.
-  exists ep1, nil; split; auto. rewrite H. simpl. auto.
-  monadInv H. 
-  edestruct IHl1 as (ep2 & y & TC1 & TC2). apply EQ.
-  rewrite TC1. simpl.
-  edestruct transl_instr_eq as (ti & TI & EQti). eauto. subst.
-  generalize (transl_instr_eq' _ _ _ _ y _ TI). simpl. intro TI2.
-  rewrite TI2.
-  monadInv TC2.
-  eexists _, _; split. eauto.
-  rewrite EQ1. simpl. rewrite app_ass. reflexivity.        
-Qed.
-
 Lemma code_tail_code_size:
   forall a b sz,
     code_tail sz (a ++ b) b ->
@@ -1197,7 +933,7 @@ Opaque loadind.
   assert (rs0 x0 = Vptr f' Ptrofs.zero).
     exploit ireg_val; eauto. rewrite H0; intros LD; inv LD; auto.
   generalize (code_tail_next_int _ _ _ _ NOOV H7). intro CT1.
-  set (sz:=(Ptrofs.repr (instr_size ((Pcall_r x0 sig))))).
+  set (sz:=(Ptrofs.repr (instr_size ((Pcall (inl x0) sig))))).
   assert (TCA: transl_code_at_pc ge (Vptr fb (Ptrofs.add ofs sz)) fb f c false tf x).
     econstructor; eauto.
   exploit return_address_offset_correct; eauto. intros; subst ra.
@@ -1218,14 +954,15 @@ Opaque loadind.
 
 + (* Direct call *)
   generalize (code_tail_next_int _ _ _ _ NOOV H7). intro CT1.
-  set (sz:=(Ptrofs.repr (instr_size ((Pcall_s fid sig))))).
+  set (sz:=(Ptrofs.repr (instr_size ((Pcall (inr fid) sig))))).
   assert (TCA: transl_code_at_pc ge (Vptr fb (Ptrofs.add ofs sz)) fb f c false tf x).
     econstructor; eauto.
   exploit return_address_offset_correct; eauto. intros; subst ra.
   left; econstructor; split.
   apply plus_one. eapply exec_step_internal. eauto.
   eapply functions_transl; eauto. eapply find_instr_tail; eauto.
-  unfold exec_instr; simpl. unfold Genv.symbol_address. rewrite symbols_preserved. rewrite H. eauto.
+  unfold exec_instr; simpl. unfold Genv.symbol_address. rewrite symbols_preserved. rewrite H. simpl. rewrite pred_dec_true; auto.
+  edestruct @Genv.find_funct_ptr_transf_partial as (tf0 & FFP' & TR). eauto. 2: rewrite FFP'. eauto. eauto.
   econstructor; eauto.
   econstructor; eauto.
   apply Mem.extends_push; auto.
@@ -1362,12 +1099,14 @@ exploit functions_translated. apply FFPcalled. intros (tf1 & FPPcalled' & TF).
   apply frame_size_correct in FIND. rewrite <- FIND. auto. 
   rewrite <- H5. simpl. eauto.
   eapply functions_transl; eauto. eapply find_instr_tail; eauto.
-  unfold exec_instr; simpl. eauto. traceEq.
+  unfold exec_instr; simpl.
+  unfold Genv.symbol_address. rewrite symbols_preserved. rewrite H. simpl. rewrite pred_dec_true; auto.
+  edestruct @Genv.find_funct_ptr_transf_partial as (tf2 & FFP' & TR). eauto. 2: rewrite FFP'. eauto. eauto.
+  traceEq.
   econstructor; eauto.
   apply agree_set_other; auto. apply agree_nextinstr. apply agree_set_other; auto.
   repeat rewrite_stack_blocks. simpl. rewrite <- H14. simpl. inversion 1. subst. rewrite EQsp. simpl.
   eapply agree_change_sp; eauto. congruence. constructor.
-  rewrite Pregmap.gss. unfold Genv.symbol_address. rewrite symbols_preserved. rewrite H. auto.
   repeat rewrite_stack_blocks; intros; repeat rewrite_perms; eauto.
   destr. apply SAMEPERM. rewrite in_stack_cons in H0. destruct H0. easy. apply in_stack_tl. rewrite EQ1; simpl; auto.
   repeat rewrite_stack_blocks. rewrite SAMEADT. intros A B; rewrite A in B; inv B; auto.
@@ -1741,6 +1480,8 @@ Proof.
   - econstructor.
     eapply (Genv.init_mem_transf_partial TRANSF); eauto.
     eauto.
+    rewrite (match_program_main TRANSF).
+    rewrite symbols_preserved. eauto.
   - replace (Genv.symbol_address (Genv.globalenv tprog) (prog_main tprog) Ptrofs.zero)
     with (Vptr fb Ptrofs.zero).
     + split. econstructor; eauto.
